coq/denot/properties.v
@@ -1,0 +1,478 @@
+Require Import Coq.Logic.FunctionalExtensionality.
+Require Import Coq.Classes.RelationClasses.
+Require Coq.Relations.Relation_Definitions.
+Require Import Lia.
+
+Require Export lc.tactics.
+Require Import structures.Structures.
+Require Export structures.consistency.
+
+
+Import MonadNotation.
+Open Scope monad_scope.
+Import SetNotations.
+Local Open Scope set_scope.
+
+
+Definition monotone {A}{B} (F : P A -> P B) : Set := 
+  forall D1 D2, (D1 ⊆ D2) -> F D1 ⊆ F D2.
+
+(* aka sub_preserving *)
+Definition sub_reflecting {A}{B} (F : P A -> P B) : Set := 
+  forall D1 D2, F D1 ⊆ F D2 -> (D1 ⊆ D2).
+
+Definition finite {B} (X : P B) : Prop := 
+  exists E, (X ≃ mem E) /\ nonempty_fset E.
+
+
+Definition continuous {V}{A} (F : P V -> P A) : Set :=
+  forall X E, mem E ⊆ F X -> valid X 
+         -> exists D, (mem D ⊆ X) /\ ((mem E) ⊆ F (mem D)) /\ valid_mem D.
+
+
+
+(* ------------ environments ---------------------- *)
+
+Ltac gather_atoms ::=
+  let A := gather_atoms_with (fun x : vars => x) in
+  let B := gather_atoms_with (fun x : var => {{ x }}) in
+  let C := gather_atoms_with (fun x => fv_tm x) in
+  let D := gather_atoms_with (fun x : list (atom * P _) => dom x) in
+  let E := gather_atoms_with (fun x : Env _ => dom x) in
+  constr:(A \u B \u C \u D \u E).
+
+
+Module EnvNotations.
+Notation "ρ ⋅ x" := (Env.access (fun x => False) ρ x) (at level 50).
+Infix "⊔e" := (Env.map2 Union) (at level 60).
+Infix "⊆e" := (Env.Forall2 Included) (at level 50).
+Infix "≃e" := (Env.Forall2 Same_set) (at level 60).
+End EnvNotations.
+
+Import EnvNotations.
+
+
+Section EnvProperties.
+
+Context {Value : Type}.
+
+Definition Rho V := Env (P V).
+
+Definition Bottom : P Value := fun x => False.
+
+Definition monotone_env {A} (XS: atoms) (D : Rho Value -> P A) := 
+  forall ρ ρ' , dom ρ [=] XS -> ρ ⊆e ρ' -> (D ρ) ⊆ D ρ'.
+
+Definition finite_env : Rho Value -> Prop := Env.Forall finite.
+  
+Definition nonempty_env : Rho Value -> Type := Env.ForallT nonemptyT.
+
+Definition sub_env : Rho Value -> Rho Value -> Prop := Env.Forall2 Included.
+
+Definition same_env : Rho Value -> Rho Value -> Prop := Env.Forall2 Same_set.
+
+
+Definition continuous_In {A} (D:Rho Value -> P A) (ρ:Rho Value) (v:A) : Prop :=
+  v ∈ D ρ -> exists ρ' , exists (pf : finite_env ρ'),  ρ' ⊆e ρ /\ (v ∈ D ρ').
+
+Definition continuous_env {A} (D:Rho Value -> P A) (ρ:Rho Value) : Prop :=
+  forall (v : A), continuous_In D ρ v.
+
+Definition continuous_Sub {A} (D:Rho Value -> P A) (ρ:Rho Value) (V:fset A) : Prop :=
+  mem V ⊆ D ρ -> 
+  exists ρ', exists (pf : finite_env ρ'),
+    ρ' ⊆e ρ  /\ (mem V ⊆ D ρ').
+
+End EnvProperties.
+
+Section EnvResults.
+
+Context {Value : Type}.
+
+(* Nonempty environments *)
+
+Lemma extend_nonempty_env {ρ : Rho Value}{x X} : 
+  x `notin` dom ρ ->
+  nonemptyT X -> 
+  nonempty_env ρ -> nonempty_env (x ~ X ++ ρ).
+Proof. intros Fr NEP NEX. eapply ForallT_cons; eauto. Qed.
+
+
+Lemma join_finite_env {ρ1 ρ2 : Rho Value} : 
+  same_scope ρ1 ρ2 
+  -> finite_env ρ1
+  -> finite_env ρ2
+  -> finite_env (ρ1 ⊔e ρ2).
+Proof.
+  move: ρ2.
+  induction ρ1 as [|[x1 v1] r1].
+  all: intros ρ2 sc h1; destruct ρ2 as [|[x2 v2] r2]; intros h2; simpl; eauto.
+  inversion h1; subst; clear h1.
+  inversion h2; subst; clear h2.
+  destruct (x1 == x2); subst.
+  + econstructor; eauto. eapply IHr1; eauto. inversion sc. auto.
+    rewrite sub_dom1; auto.
+    match goal with 
+    | [ H4 : finite v1 |- _ ] =>  destruct H4 as [E1 [s1 u1 ]] end.
+    match goal with 
+    | [ H4 : finite v2 |- _ ] =>  destruct H4 as [E2 [s2 u2 ]] end.
+    exists (union_fset E1 E2).
+    split.
+    rewrite -> s1.
+    rewrite -> s2.
+    rewrite union_mem. reflexivity.
+    eauto.
+  + assert False. inversion sc. subst. done. done.
+Qed.
+
+Lemma join_lub {ρ ρ1 : Rho Value} :
+  same_scope ρ1 ρ ->
+  forall ρ2, same_scope ρ2 ρ ->
+  ρ1 ⊆e ρ -> ρ2 ⊆e ρ -> (ρ1 ⊔e ρ2) ⊆e ρ.
+Proof.
+  intro SS1.
+  induction SS1; intros ρ2 SS2; inversion SS2; subst.
+  simpl. auto.
+  intros.
+  simpl.
+  inversion H1. inversion H2. subst.
+  rewrite eq_dec_refl.
+  eapply Env.Forall2_cons; eauto.
+  rewrite sub_dom1. auto.
+  rewrite -> H21.
+  rewrite -> H13.
+  rewrite union_idem.
+  reflexivity.
+Qed.
+  
+Lemma join_sub_left {ρ1 ρ2 : Rho Value} : 
+  same_scope ρ1 ρ2 ->
+  ρ1 ⊆e (ρ1 ⊔e ρ2).
+Proof.
+  intros h.
+  induction h; simpl; eauto.
+  rewrite eq_dec_refl.
+  econstructor; eauto. 
+Qed.
+
+Lemma join_sub_right {ρ1 ρ2 : Rho Value} : 
+  same_scope ρ1 ρ2 ->
+  ρ2 ⊆e (ρ1 ⊔e ρ2).
+Proof.
+  induction 1; simpl; eauto. 
+  rewrite eq_dec_refl.
+  econstructor; eauto. 
+  erewrite Forall2_dom in H0; eauto.
+Qed.
+
+Definition initial_finite_env (ρ : Rho Value) (NE : nonempty_env ρ) : Rho Value.
+  induction NE. exact nil.
+  destruct f as [V _].
+  exact (cons (x, ⌈ V ⌉) IHNE).
+Defined.
+
+Lemma initial_finite_dom : forall E NE, dom (initial_finite_env E NE) = dom E.
+Proof.
+  induction NE; simpl. auto.
+  destruct f as [v w].  simpl. congruence.
+Qed. 
+
+Lemma finite_singleton : forall {B} (v : B), finite ⌈ v ⌉.
+Proof. intros B v. exists (singleton_fset v).
+       repeat split; eauto. done. 
+Qed.
+
+
+
+Lemma initial_fin (ρ : Rho Value) (NE : nonempty_env ρ) :
+  finite_env (initial_finite_env ρ NE).
+Proof.
+  induction NE.
+  simpl. econstructor.
+  simpl. destruct f as [v w1 ].
+  econstructor; eauto.
+  rewrite initial_finite_dom. auto.
+  eapply finite_singleton.
+Qed.
+
+Lemma initial_fin_sub (ρ : Rho Value) (NE : nonempty_env ρ) :
+  initial_finite_env ρ NE ⊆e ρ.
+Proof.
+  induction NE; simpl. econstructor.
+  destruct f as [v fx].
+  econstructor. auto.
+  rewrite initial_finite_dom. auto.
+  intros z y. inversion y. subst. unfold In. auto.
+Qed.
+
+
+(* single-env maps x to D and any other variable y to something in ρ y. *)
+Definition single_env (x : atom) (D : P Value) (ρ : Rho Value) 
+  (NE : nonempty_env ρ) : Rho Value :=
+  update x D (initial_finite_env ρ NE).
+
+  
+Lemma single_fin { X x ρ NE } : 
+  finite X ->
+  finite_env (single_env x X ρ NE).
+Proof.
+  induction NE; intro FIN; unfold finite_env; eauto.
+  unfold single_env; econstructor.
+  unfold single_env. simpl. 
+  destruct f as [v1 v2].
+  destruct (x == x0) eqn:EQ.
+  + subst. rewrite update_eq_var. 
+    econstructor.
+    eapply initial_fin. simpl_env. auto.
+    rewrite initial_finite_dom. auto.
+    auto.
+  + rewrite update_neq_var; eauto.
+    econstructor; eauto.
+    eapply IHNE; eauto.
+    simpl_env. rewrite initial_finite_dom. auto.
+    eapply finite_singleton.
+Qed.
+
+
+
+
+Lemma single_sub { ρ x V } :
+  forall (NE : nonempty_env ρ),
+    V ⊆ ρ ⋅ x 
+  -> x `in` dom ρ
+  -> (single_env x V ρ NE) ⊆e ρ.
+Proof.
+  intros NE.
+  induction NE.
+  all: intros vpe Indom. 
+  + (* nil case *) cbn. eauto.
+    
+  + (* cons case *)
+    unfold single_env in *.
+    simpl. simpl_env in Indom.
+    destruct f as [w h2]. simpl.
+    simpl in vpe.
+    destruct (x == x0).
+    ++ subst. econstructor; eauto.
+       simpl_env. eapply initial_fin_sub. rewrite initial_finite_dom. eauto.
+    ++ econstructor; eauto. 
+       eapply IHNE; eauto. fsetdec.
+       simpl_env. rewrite initial_finite_dom. auto.
+Qed.
+
+
+
+Lemma update_access : forall {x ρ NE X},
+  x `in` dom ρ ->
+  X ≃ (single_env x X ρ NE) ⋅ x.
+Proof.
+  intros.
+  unfold single_env.
+  move: NE.
+  induction NE. fsetdec.
+  simpl. destruct f as [w h2]. simpl.
+  destruct (x == x0) eqn:EQ. subst. simpl.
+  rewrite eq_dec_refl. reflexivity.
+  simpl. rewrite EQ. eapply IHNE; auto. simpl in H. fsetdec.
+Qed.  
+
+
+
+(* v∈single[xv]x  *)
+Lemma v_single_xvx {v x ρ NE} : 
+  x `in` dom ρ ->
+  v ∈ (single_env x ⌈ v ⌉ ρ NE ⋅ x).
+Proof.
+  unfold single_env.
+  move: NE.
+  induction NE; intro h. fsetdec.
+  simpl. destruct f as [w h2]. simpl.
+  destruct (x == x0) eqn:EQ. subst. simpl.
+  rewrite eq_dec_refl. econstructor; eauto.
+  simpl. rewrite EQ. simpl in h. eapply IHNE; auto. fsetdec.
+Qed.  
+
+(* continuous-∈⇒⊆ *)
+Lemma continuous_In_sub {A} (E : Rho Value -> (P A)) ρ (NE : nonempty_env ρ) :
+   monotone_env (dom ρ) E
+   -> forall V, mem V ⊆ E ρ
+   -> (forall v, v ∈ mem V -> continuous_In E ρ v)
+   -> exists ρ', exists (pf : finite_env ρ') ,  ρ' ⊆e ρ /\ (mem V ⊆ E ρ').
+Proof.
+  intros me VS.
+  eapply fset_induction with (f := VS).
+  Unshelve. 3: exact VS.
+  - move=> VE vcont.
+    exists (initial_finite_env ρ NE).
+    repeat split.
+    eapply (initial_fin ρ NE).
+    eapply initial_fin_sub; eauto. 
+    done.
+  - move=> a f IHVS VE vcont.
+    rewrite union_mem in VE.
+    destruct IHVS as [ ρ1 [ fρ1 [ ρ1ρ VEρ1 ]]]; eauto.
+    move=> v vIn. eapply vcont. rewrite union_mem. eapply Union_intror. auto.
+    destruct (vcont a) as [ρ2 [fρ2 [ρ2ρ VEρ2]]].
+    rewrite union_mem. econstructor; eauto. rewrite mem_singleton_eq. eauto.
+    eapply VE. econstructor; eauto. 
+    rewrite mem_singleton_eq. eauto.
+    exists (ρ1 ⊔e ρ2).
+    have S1: same_scope ρ1 ρ. eapply Forall2_same_scope; eauto.
+    have S2: same_scope ρ2 ρ. eapply Forall2_same_scope; eauto. 
+    have SS: same_scope ρ1 ρ2. 
+    { transitivity ρ; auto. symmetry; auto. }
+    eexists. eapply join_finite_env; eauto.
+    repeat split.
+    + eapply join_lub; eauto.
+    + intros d dm.
+      rewrite union_mem in dm.
+      rewrite mem_singleton_eq in dm.
+      inversion dm; subst.
+      eapply me with (ρ := ρ2). admit. eapply join_sub_right; eauto. inversion H. subst. auto.
+      eapply me with (ρ := ρ1). admit. eapply join_sub_left; eauto. auto.
+Admitted.
+
+
+Lemma access_continuous_env { ρ x } : 
+  nonempty_env ρ -> continuous_env (fun ρ0 : Rho Value => ρ0 ⋅ x) ρ.
+Proof. 
+  move=> NE v vIn.
+  cbn in vIn.
+  destruct (FSetDecideAuxiliary.dec_In x (dom ρ)).
+  exists (single_env x ⌈ v ⌉ ρ NE).
+  repeat split.
+  eapply single_fin; eauto.
+  eapply finite_singleton; eauto.
+  eapply single_sub; auto.
+  eapply v_single_xvx; eauto.
+  exists (initial_finite_env ρ NE).
+  rewrite access_fresh in vIn. auto. done.
+Qed.
+
+(* ⟦⟧-continuous-⊆ *) 
+Lemma generic_continuous_sub {A}{ρ}{F : Rho Value -> P A} : 
+    continuous_env F ρ 
+  -> monotone_env (dom ρ) F
+  -> nonempty_env ρ
+  -> forall V, mem V ⊆ F ρ
+  -> exists ρ', exists (pf : finite_env ρ'),
+        ρ' ⊆e ρ  /\  (mem V ⊆ F ρ').
+Proof.
+  intros Fcont Fmono NE_ρ V VinEρ.
+  eapply continuous_In_sub; eauto.
+Qed.
+
+
+End EnvResults.
+
+#[export] Hint Resolve extend_nonempty_env : core.
+#[export] Hint Resolve single_sub : core. 
+#[export] Hint Resolve single_fin : core. 
+#[export] Hint Resolve initial_fin_sub : core. 
+#[export] Hint Resolve initial_fin : core. 
+#[export] Hint Resolve finite_singleton : core. 
+#[export] Hint Rewrite @initial_finite_dom : rewr_list.
+#[export] Hint Resolve v_single_xvx : core. 
+
+
+(* Sub environments ⊆e *)
+
+Section EnvCongruence.
+
+Context {Value : Type}.
+
+Lemma Reflexive_sub_env {ρ:Env (P Value)} : uniq ρ -> ρ ⊆e ρ.
+Proof.
+  intros. eapply Env.Forall2_refl; eauto.
+  typeclasses eauto.
+Qed.
+
+Lemma extend_sub_env {ρ ρ': Env (P Value)}{y X} :
+  y `notin` dom ρ ->
+  ρ ⊆e ρ' -> (y ~ X ++ ρ) ⊆e (y ~ X ++ ρ' ).
+Proof. intros; econstructor; eauto. reflexivity. Qed.
+
+Lemma access_mono_sub : forall (ρ1 ρ2 : Env (P Value)) (x : atom),
+   ρ1 ⊆e ρ2 ->
+   ρ1 ⋅ x ⊆ ρ2 ⋅ x.
+intros. 
+destruct (FSetDecideAuxiliary.dec_In  x (dom ρ1)).
+    + apply Forall2_access with (f := Included); auto.
+    + rewrite access_fresh. auto.
+      rewrite access_fresh. erewrite Forall2_dom in H0; eauto.
+      reflexivity.
+Qed. 
+
+Lemma same_env_sub_env : forall (x y : Env (P Value)), x ≃e y <-> (x ⊆e y) /\ (y ⊆e x).
+Proof. 
+intros x y. split.
+induction 1. split; eauto. 
+move: H1 => [s1 s2].
+move: IHForall2 => [h1 h2]. 
+split; econstructor; eauto.
+erewrite Forall2_dom; eauto.
+unfold same_env.
+intros [h1 h2]. 
+induction h1. eauto.
+inversion h2. subst.
+econstructor; eauto.
+split; auto.
+Qed. 
+
+
+End EnvCongruence.
+
+
+#[export] Instance Proper_access_sub {Value} : 
+  Proper (sub_env ==> Logic.eq ==> Included) (@access (P Value) (fun x => False)). 
+Proof.
+  intros x2 y2 S2 x3 y3 ->. eapply access_mono_sub. eauto.
+Qed.  
+
+#[export] Instance Proper_access_eq {Value} : 
+  Proper (same_env ==> Logic.eq ==> Same_set) (@access (P Value) (fun x => False)). 
+Proof.
+  intros x2 y2 EQ x3 y3 ->. 
+  apply same_env_sub_env in EQ. destruct EQ as [S1 S2].
+  split; eapply access_mono_sub; eauto.  
+Qed.  
+
+#[export] Instance Transitive_sub_env {Value}  : 
+  Transitive (@Env.Forall2 (P Value) (P Value) Included).
+Proof. typeclasses eauto. Qed.
+
+#[export] Hint Resolve Reflexive_sub_env : core.
+#[export] Hint Resolve extend_sub_env : core.
+
+
+(* valid sets are inhabited *)
+Definition valid_is_nonempty {A} (V : P A) : valid V -> nonemptyT V := id.
+
+Lemma valid_join : forall {A} ( v1 v2 : P A), 
+    valid v1 -> 
+    valid v2 ->
+    valid (v1 ∪ v2).
+Proof.
+  intros A v1 v2 [x1 h1] [x2 h2].
+  exists x1. eapply Union_introl; eauto.
+Qed.
+
+Section ValidTheory.
+
+Context {Value : Type}.
+
+Lemma valid_nil : @nonempty_env Value nil.
+Proof. unfold nonempty_env. eauto. Qed.
+
+
+Lemma extend_valid_env {ρ : Env (P Value)}{x X} : 
+  x `notin` dom ρ ->
+  valid X -> 
+  nonempty_env ρ -> nonempty_env (x ~ X ++ ρ).
+Proof. intros Fr NEP NEX.  eapply ForallT_cons; eauto. Qed.
+
+End ValidTheory.
+
+#[export] Hint Resolve valid_nil : core.
+#[export] Hint Immediate valid_is_nonempty : core.
+#[export] Hint Resolve extend_valid_env : core.
