coq/simple/model.v
@@ -1,0 +1,611 @@
+
+
+Require Import Coq.Logic.FunctionalExtensionality.
+Require Import Coq.Classes.RelationClasses.
+Require Coq.Relations.Relation_Definitions.
+Require Import Lia.
+
+Require Export lc.tactics.
+Require Export lc.scoped.
+Require Import structures.Structures.
+Require Export structures.consistency.
+
+Require Export denot.properties.
+
+Import MonadNotation.
+Open Scope monad_scope.
+Import SetNotations.
+Local Open Scope set_scope.
+
+(* This is an  example of the graph model for the pure 
+   untyped lambda calculus. 
+
+   In this model, everything is a function.
+   
+*)
+
+
+(* ----------------------------------------------------------- *)
+
+
+(* The denotation of a lambda calculus function is as its "graph" or set of
+   input / output pairs.
+   
+   Each pair in the set (i.e. v_map VS W) declares that if this value is
+   applied to any value in VS, the result is W.
+   
+   
+
+ *)
+
+Inductive Value : Type :=
+
+  (* one entry in a function's table. The first argument is the input. The second in the output. *)
+  | v_map : fset Value -> Value -> Value
+
+  (* trivial function value, evaluated to a value but never applied *)
+  | v_fun : Value.
+
+#[export] Hint Constructors Value : core.
+
+
+(* semantic operators *)
+
+Definition LAMBDA : (P Value -> P Value) -> P Value :=
+  fun f => fun v => match v with 
+          | v_map V w => (w ∈ (f (mem V))) /\ valid_mem V  (* CBV *)
+          | v_fun => True
+          end.
+
+Inductive APPLY : P Value -> P Value -> Value -> Prop :=
+  | BETA : forall D1 D2 w V,
+     (v_map V w) ∈ D1 ->
+     (mem V ⊆ D2) -> valid_mem V ->
+     APPLY D1 D2 w.
+
+(* Denotation function *)
+
+Import EnvNotations.
+Import LCNotations.
+
+Open Scope tm.
+
+Definition Rho := Env (P Value).
+
+Ltac gather_atoms ::=
+  let A := gather_atoms_with (fun x : vars => x) in
+  let B := gather_atoms_with (fun x : var => {{ x }}) in
+  let C := gather_atoms_with (fun x => fv_tm x) in
+  let D := gather_atoms_with (fun x : list (atom * P Value) => dom x) in
+  let E := gather_atoms_with (fun x : Env (P Value) => dom x) in
+  constr:(A \u B \u C \u D \u E).
+
+(* Denotation function *)
+(* `n` is is a termination metric. *)
+Fixpoint denot_n (n : nat) (a : tm) (ρ : Rho) : P Value :=
+  match n with
+  | O => Bottom
+  | S m => 
+     match a with 
+     | var_b _ => Bottom
+
+     | var_f x => ρ ⋅ x 
+
+     | abs t => 
+        let x := fresh_for (dom ρ \u fv_tm t) in 
+        (LAMBDA (fun D => (denot_n m (t ^ x) (x ~ D ++ ρ))))
+
+     | app t u   => 
+          APPLY (denot_n m t ρ) (denot_n m u ρ)
+
+     | _ => Bottom
+     end
+end.
+
+Definition denot a := denot_n (size_tm a) a.
+
+
+Lemma denot_var_b : forall x ρ, denot (var_b x) ρ = Bottom.
+Admitted.
+
+Lemma denot_var : forall x ρ, denot (var_f x) ρ = (ρ ⋅ x).
+Admitted.
+
+Lemma denot_app : forall t u ρ, 
+    denot (app t u) ρ = APPLY (denot t ρ) (denot u ρ).
+Admitted.
+
+
+Lemma denot_abs : forall x t ρ,
+    x `notin` dom ρ \u fv_tm t ->
+    denot (abs t) ρ = LAMBDA (fun D => denot (t ^ x) (x ~ D ++ ρ)).
+Admitted.
+
+Create HintDb denot.
+#[export] Hint Opaque denot : denot.
+#[export] Hint Rewrite denot_var_b denot_var denot_app : denot.
+
+
+(* --------------- monotonicity ------------------------------ *)
+
+(* Λ-ext-⊆  *)
+
+(* NOTE: By restricting the hypothesis to only valid sets, we strengthen 
+   the result. But this depends on the definition of Λ which quantifies
+   over valid sets (i.e. CBV) *)
+Lemma LAMBDA_ext_sub {F1 F2} :
+  (forall {X : P Value}, valid X -> F1 X ⊆ F2 X) -> LAMBDA F1 ⊆ LAMBDA F2.
+Proof.
+  intros F1F2 v Iv. destruct v eqn:E; inversion Iv; auto.
+  - split; auto. 
+    eapply F1F2; eauto. 
+Qed.
+
+Lemma LAMBDA_ext {F1 F2} :
+  (forall {X}, valid X -> F1 X ≃ F2 X) -> LAMBDA F1 ≃ LAMBDA F2.
+Proof. 
+  intros g. split;
+  eapply LAMBDA_ext_sub; intros X NEX; destruct (g X); eauto.
+Qed.
+
+Lemma APPLY_mono_sub { D1 D2 D3 D4 } :
+    D1 ⊆ D3 -> D2 ⊆ D4 -> ((APPLY D1 D2) ⊆ (APPLY D3 D4)).
+Proof.  
+  intros D13 D24 w APP. 
+  inversion APP; subst; unfold Included in *.
+  apply BETA with (V:=V); eauto.
+    intros d z. eauto.
+Qed.
+
+Lemma APPLY_cong { D1 D2 D3 D4 } :
+    D1 ≃ D3 -> D2 ≃ D4 -> ((APPLY D1 D2) ≃ (APPLY D3 D4)).
+Proof.
+  intros [ d13 d31 ] [ d24 d42 ].
+  split; eapply APPLY_mono_sub; eauto.
+Qed.
+
+#[export] Instance Proper_Included_APPLY : Proper (Included ==> Included ==> Included) APPLY. 
+unfold Proper. intros x1 y1 E1 x2 y2 E2. eapply APPLY_mono_sub; eauto. Qed.
+
+#[export] Instance Proper_Same_APPLY : Proper (Same_set ==> Same_set ==> Same_set) APPLY. 
+unfold Proper. intros x1 y1 E1 x2 y2 E2. eapply APPLY_cong; eauto. Qed.
+
+(* denot *)
+
+#[export] Instance Proper_sub_denot : Proper (eq ==> Env.Forall2 Included ==> Included) denot.
+Proof.
+  intros t1 t ->.
+  eapply tm_induction with (t := t).
+  1: move=>i.
+  2: move=>x.
+  3: move=>t1 t2 IH1 IH2.
+  4: move=> t' IH.
+  all: intros.
+  all: try move=> ρ1 ρ2 SUB.
+  all: autorewrite with denot.
+  all: try reflexivity.
+  - eapply access_mono_sub; eauto.
+  - eapply APPLY_mono_sub; eauto.
+  - pick fresh x.
+    repeat rewrite(denot_abs x); try fsetdec.
+    eapply LAMBDA_ext_sub; eauto.
+    move=> X neX.
+    eapply IH; eauto.
+Qed.
+
+(* The denotation respects ≃ *)
+#[export] Instance Proper_denot : Proper (eq ==> same_env ==> Same_set) denot.
+Proof.
+  intros t1 t -> x y E.
+  unfold same_env in E.
+  rewrite same_env_sub_env in E. destruct E. 
+  split; eapply Proper_sub_denot; auto. 
+Qed. 
+
+(*  forall ρ ρ', ρ ⊆e ρ' -> denot t ρ ⊆ denot t ρ'. *)
+Lemma denot_monotone {t}: forall (scope : atoms), 
+  monotone_env scope (denot t).
+Proof.
+  unfold monotone_env.
+  intros. 
+  eapply Proper_sub_denot; auto.
+Qed.
+
+(* -- monotonicity WRT argument -- *)
+
+(* denot-monotone-one *)
+Lemma denot_monotone_one : forall ρ t x, 
+    uniq ρ -> x `notin` dom ρ ->
+    monotone (fun D => denot (t ^ x) (x ~ D ++ ρ)).
+Proof. 
+  intros.
+  unfold monotone. 
+  intros D1 D2 sub.
+  eapply denot_monotone with (scope := {{x}} \u dom ρ); simpl; auto.
+  fsetdec.
+  econstructor; eauto.
+Qed.
+
+
+(* ------------------ valid ---------------------- *)
+
+Lemma valid_LAMBDA : forall F, valid (LAMBDA F).
+Proof. 
+  intros F. 
+  cbv.
+  exists v_fun. auto. 
+Qed.
+
+(* ------------------ continuity ---------------------- *)
+
+
+Lemma APPLY_continuous_env {D E : Rho -> P Value}{ρ} :
+  (nonempty_env ρ)
+  -> continuous_env D ρ 
+  -> continuous_env E ρ
+  -> monotone_env (dom ρ) D 
+  -> monotone_env (dom ρ) E
+  -> continuous_env (fun ρ => APPLY (D ρ)(E ρ)) ρ.
+Proof.  
+  intros NE IHD IHE mD mE.
+  intros w APP.
+  inversion APP; subst.
+  destruct (IHD (v_map V  w ) ltac:(auto)) as 
+      [ ρ1 [ fρ1 [ ρ1ρ VwDp1 ]]].
+  destruct 
+      (continuous_In_sub E ρ NE mE V)
+      as [ ρ2 [ fρ2 [ ρ2ρ VEp2 ]]]; eauto.
+  have S1: same_scope ρ1 ρ. eapply Forall2_same_scope; eauto.
+  have S2: same_scope ρ2 ρ. eapply Forall2_same_scope; eauto.
+  have SS: same_scope ρ1 ρ2. { transitivity ρ; auto. symmetry; auto. }
+  exists (ρ1 ⊔e ρ2).
+  repeat split.
+    -- eapply join_finite_env; eauto.
+    -- eapply join_lub; eauto.
+    -- have VwDp3 : ⌈ v_map V w ⌉ ⊆ D (ρ1 ⊔e ρ2).
+    { transitivity (D ρ1); auto. eapply mD. 
+      erewrite -> Env.Forall2_dom with (r2 := ρ); eauto. reflexivity.
+      eapply join_sub_left. auto. }
+    have VEρ3 : mem V ⊆ E (ρ1 ⊔e ρ2).
+    { transitivity (E ρ2); auto. eapply mE.
+      erewrite -> Env.Forall2_dom with (r2 := ρ); eauto. reflexivity.
+      eapply join_sub_right.  auto. }
+    eapply BETA with (V:=V); auto.
+Qed.
+
+(* Algebraicity.  
+   Only need finite information from the environment.
+*)
+
+Lemma LAMBDA_continuous_env {E ρ x} {NE : nonempty_env ρ} :
+    x `notin` dom ρ
+  -> (forall V, valid_mem V -> continuous_env E (x ~ mem V ++ ρ))
+  -> monotone_env ({{x}} \u (dom ρ)) E
+  -> continuous_env (fun ρ => LAMBDA (fun D => E (x ~ D ++ ρ))) ρ.
+Proof.
+  intros Fr IH mE.
+  intros v vIn.
+  destruct v; try done.
+  - (* v is l ↦ c *)
+    move: vIn => [ wEVρ NW ]. 
+    have VV: valid_mem f. unfold valid_mem. eauto.
+    have NEx: nonempty_env (x ~ mem f ++ ρ). econstructor; eauto.
+    specialize (IH f ltac:(eauto) v wEVρ).
+    destruct IH as [ρ' [F' [S' h']]].
+    inversion S'. subst. inversion F'. subst.
+    exists E1. eexists. eauto.
+    repeat split; auto.
+    eapply mE with (ρ := x ~ a1 ++ E1); simpl_env; eauto. 
+    move: (Env.Forall2_dom _ H3) => EQ. rewrite EQ. reflexivity.
+    econstructor; eauto. eapply Reflexive_sub_env. eapply Forall2_uniq1; eauto.
+  - exists (initial_finite_env ρ NE).
+    repeat split; eauto.
+Qed.
+
+
+(* ⟦⟧-continuous *)
+Lemma denot_continuous_env {t} : forall ρ,
+    nonempty_env ρ
+  -> continuous_env (denot t) ρ.
+Proof.
+  eapply tm_induction with (t := t).
+  1: move=>i ρ NE.
+  2: move=>x ρ NE.
+  3: move=>t1 t2 IH1 IH2 ρ NE.
+  4: move=> t' IH ρ NE.
+  all: intros.
+  all: intros c cIn.
+  all: autorewrite with denot in cIn.
+  all: try solve [destruct c; try done].  
+  - (* var case *)
+    eapply access_continuous_env; eauto.
+  - (* app *)
+    specialize (IH1 _ NE).
+    specialize (IH2 _ NE).
+    move: (APPLY_continuous_env NE IH1 IH2 (denot_monotone (dom ρ)) (denot_monotone (dom ρ)) c cIn) => [r1 [f1 h]].
+    exists r1. exists f1. autorewrite with denot.
+    eauto.
+  - (* abs *)
+    pick fresh x.
+    rewrite (denot_abs x) in cIn; auto. 
+    specialize (IH x ltac:(auto)).
+    destruct (@LAMBDA_continuous_env (denot (t' ^ x)) ρ x NE ltac:(auto) ltac:(eauto)
+          ltac:(eauto using denot_monotone) _ cIn) as [ρ' [F' [S' I']]].
+    exists ρ'. exists F'. 
+    rewrite (denot_abs x). 
+    erewrite -> Forall2_dom with (r2 := ρ). fsetdec. eauto.
+    eauto.    
+Qed.
+
+(* --------------------------------------------------- *)
+
+
+
+(* ⟦⟧-continuous-⊆ *) 
+Lemma denot_continuous_sub {ρ t} : 
+  nonempty_env ρ
+  -> forall V, mem V ⊆ denot t ρ
+  -> exists ρ', exists (pf : finite_env ρ'),
+        ρ' ⊆e ρ  /\  (mem V ⊆ denot t ρ').
+Proof.
+  intros NE_ρ V VinEρ.
+  eapply generic_continuous_sub;
+    eauto using denot_continuous_env, denot_monotone.
+Qed.
+
+
+(* ⟦⟧-continuous-one *)
+Lemma denot_continuous_one { t ρ x } :
+  nonempty_env ρ 
+  -> x `notin` dom ρ 
+  -> continuous (fun D => denot (t ^ x) (x ~ D ++ ρ)).
+Proof.
+  intros NE_ρ Fr.
+  intros X E E_sub_denot NE_X.
+  edestruct (@denot_continuous_sub (x ~ X ++ ρ)) as 
+    [ρ' [pf [h1 h2]]]. 3: eauto.
+  + eapply extend_nonempty_env; eauto.
+  + eauto.
+  + inversion h1. subst. inversion pf. subst.
+    match goal with [H6 : finite a1 |- _ ] => move: H6 => [D [S NN]] end.
+    exists D. split.
+    rewrite <- S. auto.
+    split. 
+    have SUB: Env.Forall2 Included 
+                (x ~ a1 ++ E1) (x ~ mem D ++ ρ).
+    econstructor; eauto. 
+    rewrite <- S. reflexivity.
+    rewrite <- SUB. eapply h2. 
+    eapply valid_sub_valid_mem; eauto. rewrite <- S. auto. 
+Qed.
+
+(*  ----- Abstraction followed by Application is the identity -------- *)
+
+(* Λ-▪-id *)
+Lemma LAMBDA_APPLY_id { F X } :
+  continuous F -> monotone F -> valid X
+  -> APPLY (LAMBDA F) X ≃ F X.
+Proof. 
+  intros Fcont Fmono NEX.
+  split.
+  + intros w APP. inversion APP; subst.
+    - cbn in H. destruct H as [h1 h2].
+      specialize (Fmono (mem V) X ltac:(auto)).
+      eauto.
+  + intros w wInFX.
+    have M: mem (singleton_fset w) ⊆ F X. 
+    { intros d y. inversion y; subst. auto. done. }
+    move: (Fcont X (singleton_fset w) M NEX) => 
+    [ D [ DltX [ wInFD NED ]]].
+    eapply BETA with (V:=D); eauto.
+    repeat split; eauto.
+Qed.
+
+
+(* Λ⟦⟧-▪-id *)
+Lemma LAMBDA_denot_APPLY_id :
+  forall t ρ x X,
+    valid X
+    -> nonempty_env ρ
+    -> x `notin` dom ρ 
+    -> (APPLY (LAMBDA (fun D => denot (t ^ x) (x ~ D ++ ρ))) X) ≃
+      denot (t ^ x) (x ~ X ++ ρ).
+Proof.
+  intros.
+  move: (@LAMBDA_APPLY_id (fun D => denot (t ^ x) (x ~ D ++ ρ)) X) => h.
+  eapply h; auto.
+  +  (* continuity *)
+    eapply denot_continuous_one; auto.
+  + eapply denot_monotone_one; auto.
+    eapply ForallT_uniq; eauto.
+Qed.
+
+(* ------------------- beta reduction is sound ----------------- *)
+
+
+Lemma subst_denot1 :
+  forall (t : tm) (x : atom) (u : tm) (ρ : Env (P Value)),
+    scoped t (x ~ denot u ρ ++ ρ) 
+    -> scoped u ρ 
+    -> valid (denot u ρ)
+    -> nonempty_env ρ
+    -> denot t (x ~ denot u ρ ++ ρ) ≃ denot (t [x ~> u]) ρ.
+Proof.
+Admitted.
+
+
+Lemma beta_soundness : forall t u ρ, 
+  scoped (abs t) ρ ->
+  scoped u ρ -> 
+  nonempty_env ρ ->
+  valid (denot u ρ) -> 
+  denot (app (abs t) u) ρ ≃ denot (open_tm_wrt_tm t u) ρ.
+Proof.
+  intros t u ρ St Su NE V.
+  pick fresh x.
+  rewrite denot_app.
+  rewrite (denot_abs x); auto.
+  rewrite (LAMBDA_denot_APPLY_id); auto.
+  rewrite subst_denot1; eauto.
+  eapply scoped_abs_inv; eauto.
+  rewrite (subst_tm_intro x t u); auto.
+  reflexivity.
+Qed.
+
+(* ------------------------ examples --------------------------- *)
+
+
+(* Identity function *)
+
+Definition tm_Id : tm := abs (var_b 0).
+ 
+Definition idset : P Value := 
+  fun t => match t with 
+          | v_fun => True 
+          | v_map IN OUT => OUT ∈ mem IN 
+        end.
+
+Definition id0 := v_fun.
+Example example0 : id0 ∈ idset. done. Qed.
+Definition id1 := v_map (FSet (id0 :: nil) ) id0.
+Example example1 : id1 ∈ idset. cbn. left. done. Qed.
+Definition id2 := v_map (FSet (id0 :: id1 :: nil) ) id1.
+Example example2 : id2 ∈ idset. cbn. right. left. done. Qed.
+Definition id3 := v_map (FSet (id0 :: id1 :: id2 :: nil) ) id2.
+Example example3 : id2 ∈ idset. cbn. right. left. done. Qed.
+
+
+Lemma denot_Id1 : denot tm_Id nil ⊆ idset.
+Proof.
+  pick fresh x.
+  rewrite (denot_abs x); simpl; auto.
+  cbn. rewrite eq_dec_refl. clear x Fr.
+  + intros x xIn.
+    destruct x; try done.
+    destruct xIn as [h1 h2].
+    cbn. auto.
+Qed.
+
+Lemma denot_Id2 : idset  ⊆  denot tm_Id nil.
+Proof. 
+  pick fresh x.
+  rewrite (denot_abs x); simpl; auto.
+  cbn. rewrite eq_dec_refl. clear x Fr.
+  move=> x xIn.
+  destruct x; try done.
+  + cbn in xIn.
+    repeat split; auto. 
+    destruct f. cbn in xIn.
+    intro h. subst.
+    done.
+Qed.
+
+(* Example: constant function K -- \x. \y. x n *)
+
+Definition tm_K : tm := abs (abs (var_b 1)).  
+
+Definition K_set : P Value := 
+  fun t => match t with 
+          | v_map V1 w => valid_mem V1 /\
+              match w with 
+                | v_map V2 v => (valid_mem V2) /\ (v ∈ mem V1)
+                | v_fun => True
+              end
+          | v_fun => True
+        end.
+
+Lemma denot_K2 : K_set ⊆ denot tm_K nil.
+Proof.
+  intros v vIn.
+  unfold tm_K.
+  pick fresh x. 
+  rewrite (denot_abs x); auto.
+  destruct v; try done.
+  destruct v; cbn in vIn; try done.
+  2: { cbn. intuition. }
+  cbn.
+  rewrite eq_dec_refl.
+  remember (fresh_for (union (Metatheory.add x empty) (singleton x))) as y.
+  destruct (x == y). subst. admit. (* variable fussiness. *)
+  intuition.
+Admitted.
+
+Lemma denot_K1 : denot tm_K nil ⊆ K_set.
+Proof.
+  unfold tm_K.
+  pick fresh x. 
+  rewrite (denot_abs x); auto.
+  replace ((abs (var_b 1)) ^ x) with (abs (var_f x)). 2: { reflexivity. }
+    
+  intros v vIn.
+  destruct v; try done.
+  destruct v; try done. 2: { cbn in *. intuition. }
+  cbn in *.
+  rewrite eq_dec_refl in vIn.
+  remember (fresh_for (union (Metatheory.add x empty) (singleton x))) as z.
+  destruct (x == z). subst. admit.
+  intuition.
+Admitted.
+
+(* Delta := \x. x x *)
+
+Definition tm_Delta : tm := abs (app (var_b 0) (var_b 0)).
+
+Definition Delta_set : P Value :=
+  fun t => match t with 
+          | v_fun => True
+          | v_map f y => valid_mem f /\ exists V, (v_map V y ∈ mem f) /\ (valid_mem V) /\ (mem V ⊆ mem f)
+        end.
+
+
+Lemma denot_Delta2 : Delta_set ⊆ denot tm_Delta nil.
+Proof.
+  unfold tm_Delta.
+  pick fresh x.
+  rewrite (denot_abs x). eauto.
+  intros y yIn.
+  cbn. rewrite eq_dec_refl.
+  destruct y; try done.
+  cbn in yIn. 
+  move: yIn => [VF [V [SF [VV SV]]]]. 
+  cbn.
+  split; eauto.
+  eapply BETA;  eauto.
+Qed.
+
+Lemma denot_Delta1 : denot tm_Delta nil ⊆ Delta_set.
+Proof.
+  unfold tm_Delta.
+  pick fresh x.
+  rewrite (denot_abs x). eauto.
+  intros y yIn.
+  cbn in yIn. rewrite eq_dec_refl in yIn.
+  destruct y; try done.
+  cbn in yIn. destruct yIn as [AP VM].
+  inversion AP. subst.
+  cbn.
+  repeat split. auto.
+  exists V. repeat split; auto.
+Qed.
+
+Lemma denot_Delta : denot tm_Delta nil ≃ Delta_set.
+Proof. split. eapply denot_Delta1. eapply denot_Delta2. Qed.
+
+(* Omega := (\x. x x)(\x. x x) *)
+
+Definition tm_Omega : tm := app tm_Delta tm_Delta.
+
+Lemma denot_Omega : denot tm_Omega nil ⊆ (fun x => False).
+Proof. intros x xIn.
+       unfold tm_Omega in xIn.
+       rewrite denot_app in xIn.
+       rewrite denot_Delta in xIn.
+       inversion xIn. subst. clear xIn.
+       cbv.
+       destruct V.
+       destruct l; try done.
+       clear H1.
+       destruct H as [_ [l1 [H1 [VV1 M1]]]].       
+       destruct l1 as [[ | w l2]]; try done. clear VV1.
+       destruct H1. subst.
+Admitted.
