coq/structures/consistency.v
@@ -1,0 +1,289 @@
+Require Import Coq.Logic.FunctionalExtensionality.
+Require Import Coq.Classes.RelationClasses.
+Require Coq.Relations.Relation_Definitions.
+Require Import Lia.
+
+Require Export lc.tactics.
+Require Import structures.Structures.
+
+Class Consistency (A : Type) : Type := 
+  { Consistent : A -> A -> Prop ;
+    Inconsistent : A -> A -> Prop ;
+  }.
+
+Section List.
+
+Context 
+  { A : Type }
+  { f : A -> A -> Prop }
+  { g : A -> A -> Prop }.
+
+Definition Consistent_list := List.Forall2 f.
+Definition Inconsistent_list := fun XS YS => 
+  length XS <> length YS \/ List.Exists2 g XS YS.
+
+End List.
+
+#[export] Instance Consistency_list { A : Type } `{ Consistency A } : Consistency (list A) := 
+  { Consistent := Consistent_list (f := Consistent) ;
+    Inconsistent := Inconsistent_list (g := Inconsistent) ;
+  }.
+
+Section FSet.
+
+Context 
+  { A : Type }
+  { f : A -> A -> Prop }
+  { g : A -> A -> Prop }.
+
+Definition Consistent_fset := fun '(FSet XS) '(FSet YS) => List.Forall2_any f XS YS.
+Definition Inconsistent_fset := fun '(FSet XS) '(FSet YS) => List.Exists2_any g XS YS.
+
+End FSet.
+
+#[export] Instance Consistency_fset { A : Type}  `{ Consistency A } : Consistency (fset A) := 
+  { Consistent := Consistent_fset (f := Consistent) ;
+    Inconsistent := Inconsistent_fset (g := Inconsistent) ;
+  }.
+
+Section Computations.
+
+Context 
+  { A : Type }
+  { f : A -> A -> Prop }
+  { g : A -> A -> Prop }.
+
+Inductive ConsistentComp  : Comp A -> Comp A -> Prop :=
+  | cc_wrong : ConsistentComp c_wrong c_wrong
+  | cc_multi : forall AS BS, 
+      List.Forall2 f AS BS ->
+      ConsistentComp (c_multi AS) (c_multi BS).
+
+Inductive InconsistentComp : Comp A -> Comp A -> Prop :=
+  | i_wrong_multi : forall AS, InconsistentComp c_wrong (c_multi AS)
+  | i_multi_wrong : forall AS, InconsistentComp (c_multi AS) c_wrong
+  | i_multi : forall AS BS, 
+      (length AS <> length BS \/ List.Exists2 g AS BS) -> 
+      InconsistentComp (c_multi AS) (c_multi BS).
+
+End Computations.
+
+#[export] Instance Consistency_Comp {A:Type} `{Consistency A} : Consistency (Comp A) := 
+  { Consistent := ConsistentComp (f:=Consistent) ; Inconsistent := InconsistentComp (g := Inconsistent) }.
+
+#[export] Hint Constructors ConsistentComp InconsistentComp : core.
+
+
+Import SetNotations.
+
+(* Two sets are consistent if all of their elements 
+   are consistent. *)
+Definition ConsistentSets {A:Type} `{Consistency A} V1 V2 := 
+    forall x y, x ∈ V1 -> y ∈ V2 -> Consistent x y.
+
+Definition InconsistentSets {A:Type} `{Consistency A} V1 V2 := 
+  exists x, exists y, (x ∈ V1) /\ (y ∈ V2) /\ (Inconsistent x y).
+
+#[export] Instance Consistency_P {A:Type} `{Consistency A} : Consistency (P A) :=
+   { Consistent := ConsistentSets ; Inconsistent := InconsistentSets }.
+
+
+(* ------------------------------------------------- *)
+
+Class ConsistencyTheory (A : Type) `{Consistency A} := 
+  {  exclusive : forall x y, Consistent x y -> Inconsistent x y -> False ;
+     decidable : forall x y, {Consistent x y} + {Inconsistent x y}
+  }.
+
+Definition Exclusive {A} (f g : A -> A -> Prop) :=  forall x y, f x y -> g x y -> False .
+Definition Decidable {A} (f g : A -> A -> Prop) :=  forall x y, {f x y} + {g x y}.
+
+
+Section List.
+
+Context 
+  { A : Type }
+  { f : A -> A -> Prop }
+  { g : A -> A -> Prop }.
+
+Lemma exclusive_list :
+  Exclusive f g -> 
+  Exclusive (@Consistent_list A f) (@Inconsistent_list A g).
+Proof.
+  intros efg. intros x y FF. 
+  induction FF; intros EG; inversion EG; eauto.
+  - inversion H.
+  - move: (Forall2_length _ _ FF) => eq. 
+    simpl in H0. rewrite eq in H0. done.
+  - inversion H0; subst. eauto.
+    eapply IHFF. right. eauto.
+Qed.
+
+Lemma exclusive_list2: forall l, 
+  List.Forall (fun x : A => forall y : A, f x y -> g x y -> False) l ->
+  forall YS, (@Consistent_list A f) l YS -> (@Inconsistent_list A g) l YS -> False.
+Proof.
+  induction l; intros h YS h1 h2.
+  - inversion h1. subst. inversion h2. done.
+    inversion H.
+  - inversion h1. subst. inversion h. subst.
+    specialize (IHl H4 l' H3).
+    destruct h2. unfold Consistent_list in h1. 
+    apply Forall2_length in h1. done.
+    inversion H; subst; eauto.
+    eapply IHl. right. auto.
+Qed.    
+
+Lemma decidable_list : 
+  Decidable f g ->
+  Decidable (@Consistent_list A f) (@Inconsistent_list A g).
+Proof.
+  intros dfg. intros x.
+  induction x; intros y; destruct y.
+  - left; eauto. econstructor.
+  - right; eauto. left. done.
+  - right; eauto. left. done.
+  - destruct (IHx y). destruct (dfg a a0).
+    left. econstructor; eauto.
+    right. right. econstructor; eauto.
+    right. destruct i. left. eauto. right. eauto.
+Qed.
+
+End List.
+
+#[export] Instance Consistency_list_theory { A : Type } `{ ConsistencyTheory A } : ConsistencyTheory (list A) := 
+  { exclusive := exclusive_list (f := Consistent)(g := Inconsistent) exclusive ;
+    decidable := decidable_list (f := Consistent)(g := Inconsistent) decidable ;
+  }.
+
+Section FSet.
+
+Context 
+  { A : Type }
+  { f : A -> A -> Prop }
+  { g : A -> A -> Prop }.
+
+
+Lemma exclusive_fset :
+  Exclusive f g ->
+  Exclusive (@Consistent_fset A f) (@Inconsistent_fset A g).
+Proof.
+  intros efg. intros x. destruct x as [x].
+  induction x; intros y FF EG; destruct y as [y]; destruct y; 
+    unfold Consistent_fset, List.Forall2_any in FF;
+    unfold Inconsistent_fset, List.Exists2_any in EG.
+  - destruct EG as [x0 [y0 [h1 [h2 _]]]]. inversion h1.
+  - destruct EG as [x0 [y0 [h1 [h2 _]]]]. inversion h1.
+  - destruct EG as [x0 [y0 [h1 [h2 _]]]]. inversion h2.
+  - destruct EG as [x0 [y0 [h1 [h2 gg]]]]. 
+    specialize (FF x0 y0 h1 h2).
+    eapply efg; eauto.
+Qed.
+
+Lemma decidable_fset :
+  Decidable f g ->
+  Decidable (@Consistent_fset A f) (@Inconsistent_fset A g).
+Proof.
+  intros dfg. intros x. destruct x as [x].
+  induction x; intros y; destruct y as [y].
+     unfold Consistent_fset, List.Forall2_any;
+     unfold Inconsistent_fset, List.Exists2_any.
+  - left. done.
+  - destruct (IHx (FSet y)). 
+    + simpl in c. simpl.
+      induction y. unfold List.Forall2_any in c.
+      left. intros x0 y0 h1 h2. inversion h2. 
+      have CE: (List.Forall2_any f x y). { intros x0 y0 h1 h2. eapply c; eauto. simpl. eauto. }
+      specialize (IHy CE). destruct IHy.
+      ++ destruct (dfg a a0).
+         left.
+         { intros x0 y0 i1 i2.
+           destruct i1; destruct i2; subst. 
+           -- auto.
+           -- apply f0; eauto. simpl; auto.
+           -- apply c; eauto. simpl; auto.
+           -- apply CE; eauto.
+         }
+         right.
+         exists a. exists a0. simpl. split; auto.
+      ++ right. destruct e as [x0 [y0 [h1 [h2 h3]]]].
+         exists x0. exists y0. simpl. eauto.
+    + right. destruct i as [x0 [y0 [i1 [i2 h]]]]. 
+      exists x0. exists y0. 
+      repeat split; try right; auto. 
+Qed.
+
+Lemma exclusive_fset2: forall l, 
+  Forall_fset (fun x : A => forall y : A, f x y -> g x y -> False) l ->
+  forall YS, (@Consistent_fset A f) l YS -> (@Inconsistent_fset A g) l YS -> False.
+Proof.
+  intro l. destruct l. 
+  move=> h YS. destruct YS as [l']. simpl in *.
+  move: h l'.
+  induction l; intros h l' h1 h2;  unfold List.Forall2_any in h1; destruct h2 as [x0 [y0 [I0 [I1 IC]]]]. 
+  - inversion I0.
+  - inversion h. subst. 
+    specialize (IHl H2).
+    rewrite Forall_forall in H2.
+    destruct I0; subst.
+    -- specialize (h1 x0 y0 ltac:(left; auto) I1).
+       eauto.
+    -- eapply (IHl l').
+       intros x1 y1 I3 I4. eapply  h1. right; eauto. eauto.
+       exists x0. exists y0. repeat split; eauto.
+Qed. 
+
+(* Consistency is reflexive ?? *)
+
+End FSet.
+
+#[export] Instance ConsistencyTheory_fset { A : Type}  `{ ConsistencyTheory A } : ConsistencyTheory (fset A) := 
+  { exclusive := exclusive_fset (f := Consistent)(g := Inconsistent) exclusive ;
+    decidable := decidable_fset (f := Consistent)(g := Inconsistent) decidable ;
+  }.
+
+Section Computations.
+
+Context 
+  { A : Type }
+  { f : A -> A -> Prop }
+  { g : A -> A -> Prop }.
+
+Lemma exclusive_Comp : 
+  Exclusive f g ->
+  Exclusive (@ConsistentComp A f) (@InconsistentComp A g).
+Proof.
+  intros efg x y CC IC.
+  induction CC; inversion IC.
+  eapply exclusive_list; eauto.
+Qed.
+
+
+Lemma exclusive_Comp2: forall l, 
+  Comp.Forall (fun x : A => forall y : A, f x y -> g x y -> False) l ->
+  forall YS, (@ConsistentComp A f) l YS -> (@InconsistentComp A g) l YS -> False.
+Proof.
+  destruct l. intros.
+Admitted.
+
+Lemma decidable_Comp : 
+  Decidable f g ->
+  Decidable (@ConsistentComp A f) (@InconsistentComp A g).
+Proof.
+  intros dfg x y.
+  destruct x eqn:EX; destruct y eqn:EY.
+  - left; econstructor.
+  - right; econstructor.
+  - right; econstructor.
+  - destruct (decidable_list dfg l l0).
+    left; econstructor; eauto.
+    right; econstructor; eauto.
+Qed.
+
+
+End Computations.
+
+#[export] Instance ConsistencyTheory_Comp { A : Type}  `{ ConsistencyTheory A } : ConsistencyTheory (Comp A) := 
+  { exclusive := exclusive_Comp (f := Consistent)(g := Inconsistent) exclusive ;
+    decidable := decidable_Comp (f := Consistent)(g := Inconsistent) decidable ;
+  }.
