coq/verse/definitions_new.v
@@ -1,0 +1,465 @@
+(* Definitions related to the denotational semantics.
+
+   This version separates the denotation of computations from that of values.
+   
+   The semantic domain for values: `P Value` and for computations: `P (Comp
+   (list Value))`
+
+   The `Comp A` type is defined in `structures.Comp`. It is isomorphic to
+   `maybe (list A)`, where none is a runtime type error and the list includes
+   multiple results.  Fail is the empty list.
+
+   The type `P A` is a (potentially) infinite set, represented by its
+   characteristic function `(A -> Prop)`. The union of all of the elements of
+   the set is the complete denotation of the value/computation. (These
+   elements should be consistent with eachother.)
+
+   The denotation of both values and computations includes the empty set: the
+   denotation of an infinite loop. Therefore, some definitions include
+   the predicate
+
+      valid : P Value -> Prop
+
+   which characterizes Values that are nonempty. i.e. do not denote bottom.
+
+   We would have liked the denotation of computations to be `P (Comp (P Value))`,
+   i.e. the type `P (Comp A)` instantiated with `P Value`. This former type is
+   *almost* a monad: there are reasonable definitions of return and bind, but
+   one of the associativity laws for bind fails. This isn't necessarily fatal:
+   it just means that we have to be careful about how we represent certain
+   computations.
+
+   However, I was unable to prove continuity for the semantic operators using
+   this definition. 
+
+   So I have used the types above, and have defined the
+   Monad-like operations:
+
+      RET : P A -> P (Comp (list A))
+
+      BIND : (P (Comp (list A))) -> (P A -> P (Comp B)) -> P (Comp B)
+
+   I don't know which of the analogous monad laws these operators satisfy. 
+
+   Other semantic operators:
+
+      NAT : nat -> P Value 
+
+      ADD : P Value 
+
+      NIL : P Value 
+
+      CONS : P Value -> P Value -> P Value 
+
+      LIST : list (P Value) -> P Value
+
+      Λ : (P Value -> P (Comp (list Value))) -> P Value     
+             -- note function bodies are computations, so functions can 
+             -- produce errors or multiple results
+
+      APPLY : P Value -> P Value -> P (Comp (list Value))
+             -- application requires two (valid) values because we can use 
+             -- BIND above to sequence the computations first
+
+   Environments. An `Env A` is an association list, associating each variable with an `A`. 
+
+      This is a call-by-value language, so the environment contains the denotation of values.
+   
+       Rho := Env (P Value)
+
+   Environment Notations:
+
+       `ρ ⋅ x` -- lookup variable x in the environment, return bottom if not in domain
+
+        x ~ a ++ ρ -- extend an environment with an association.
+
+   Environment predicates:
+
+       valid_env : Rho -> Prop    
+
+       finite_env : Rho -> Prop   -- implies valid
+
+   Denotation functions (mutually defined):
+
+       denot     : tm -> Rho -> P (Comp (list Value))
+
+       denot_val : tm -> Rho -> P Value
+
+ *)
+
+
+Require Import Coq.Logic.FunctionalExtensionality.
+Require Import Coq.Classes.RelationClasses.
+Require Coq.Relations.Relation_Definitions.
+Require Import Lia.
+
+Require Export lc.tactics.
+Require Import structures.Structures.
+Require Import semantic_notions.
+Require Import QuasiMonad.
+
+Import MonadNotation.
+Open Scope monad_scope.
+Import SetNotations.
+Local Open Scope set_scope.
+
+
+(*
+Definition PP (A : Type) : Type := { V : P A |  nonempty V}.
+
+Definition PP_Singleton {A : Type} (x : A) : PP A := 
+  exist (fun V : P A => nonempty V) ⌈ x ⌉ (Inhabited_intro A ⌈ x ⌉ x in_singleton).
+
+Definition PP_In {A : Type} (s : PP A) (x : A) : Prop.
+destruct s as [x0 _]. exact (x0 x). Defined.
+
+Definition PP_Included {A : Type} (x : PP A) (y : PP A) : Prop := forall z, PP_In x z -> PP_In y z.
+
+Definition PP_Union {A : Type} (x : PP A) (y : PP A) : PP A.
+  destruct x. destruct y. exists (Union x x0). 
+  destruct n. destruct n0.
+  eapply Inhabited_intro with (x := x1).
+  econstructor. exact H.
+Defined.
+
+Definition PP_Same_set {A : Type} (x : PP A) (y : PP A) : Prop.
+  destruct x as [s _]. destruct y as [t _]. 
+  exact (Same_set s t). 
+Defined.
+  
+Declare Scope pset_scope.
+Delimit Scope pset_scope with PP.
+Bind Scope pset_scope with PP.
+
+Module PSetNotations. 
+  Notation "x ∈ s" := (PP_In s x) : pset_scope .
+  Notation "⌈ x ⌉" := (PP_Singleton x) : pset_scope.
+  Infix "⊆" := PP_Included : pset_scope.
+  Infix "∪" := PP_Union : pset_scope.
+  Infix "≃" := PP_Same_set : pset_scope.
+End PSetNotations.
+
+Import PSetNotations.
+Open Scope pset_scope.
+
+*)
+  
+(* ----------------------------------------------------------- *)
+
+Inductive Value : Type :=
+  (* natural number *)
+  | v_nat : nat -> Value
+
+  (* one entry in a function's table *)
+  | v_map : forall (x: list Value), Comp Value -> Value
+
+  (* trivial function value, evaluated to a value but never applied *)
+  | v_fun : Value
+
+  (* list/tuple of values *)
+  | v_list : list Value -> Value.
+
+(* EXAMPLE
+
+Denotation of Identity function (\x.x):  
+
+  any subset of 
+
+ { vfun } `union` 
+ { v_map (v_nat vi :: nil) (c_multi (v_nat vi) :: nil)  | for any value vi } 
+
+ *)
+
+#[export] Hint Constructors Value : core.
+
+Infix "↦" := v_map (at level 85, right associativity).
+
+(* ------------ Semantic Operators ------------------ *)
+
+Definition NAT : nat -> P Value :=
+  fun j v => match v with 
+          | v_nat k => j = k
+          | _ => False
+          end.
+
+Definition LIST : list (P Value) -> P Value  :=
+  fun DS w => 
+    match w with 
+    | v_list WS => List.Forall2 Ensembles.In DS WS
+    | _ => False
+    end.
+
+Definition NIL : P Value := ⌈ v_list nil ⌉.
+
+Definition CONS : P Value -> P Value -> P Value := 
+  fun V W x => 
+    match x with 
+    | v_list (v :: w) => (v ∈ V) /\ (v_list w ∈ W)  
+    | _ => False
+    end.
+
+Definition coerce (w : Comp Value) : Comp (vfin Value) := 
+  fmap (fun x => 
+  match w with 
+  | c_wrong => X c_wrong
+  | c_multi lw => 
+      match c with 
+    | c_wrong => False
+    | c_multi l => List.Forall2 (fun v vf => v ∈ vmem vf) w l
+    end.
+
+Definition Λ : (P Value -> P (Comp (vfin Value))) -> P Value :=
+  fun f => fun v => match v with 
+          | (V ↦ w) => (w ∈ (f (mem V))) /\ valid_mem V  (* CBV *)
+          | v_fun => True
+          | _ => False
+          end.
+
+
+(* ------------ LOGIC PROGRAMMING ----------------- *)
+
+Definition ONE (C : P (Comp (list Value))) : P Value :=
+  fun v => exists l, c_multi (ret v  :: l) ∈ C.
+
+Definition ALL (C : P (Comp (list Value))) : P Value :=
+  fun v => match v with 
+          | v_list l => c_multi (List.map ret l) ∈ C 
+          | _ => False
+        end.
+
+Definition FAIL : P (Comp (list Value)) := ⌈ c_multi nil ⌉.
+
+Definition CHOOSE (C1 : P (Comp (list Value))) (C2 : P (Comp (list Value))) : 
+  P (Comp (list Value)) := 
+  fun c => 
+    match c with 
+    | c_multi l => 
+        exists l1, exists l2, l = l1 ++ l2 /\ (c_multi l1 ∈ C1) /\ (c_multi l2 ∈ C2)
+    | _ => False
+    end.
+
+(* Fails when V and W don't unify. Returns their union when they do. *)
+(* Need to define inconsistent here.
+
+Definition UNIFY (V : P Value) (W: P Value) : P (Comp (list Value)) :=
+  fun c => match c with 
+
+        | c_multi nil => 
+            exists v, exists w, v ∈ V /\ w ∈ W /\ Inconsistent v w
+
+        | c_multi (l :: nil) => (mem l ⊆ V ∪ W) /\ l <> nil
+
+        | _ => False
+  end.
+*)    
+  
+
+(* ------------------------------------------ *)
+
+(* This definition includes all values that produce c. *)
+
+Definition EXISTS (f : P Value -> P (Comp (list Value))) : P (Comp (list Value)) :=
+  fun c => exists V, c ∈ f (mem V).
+
+(* ------------ APPLY ----------------- *)
+
+(* It is a little easier to specify this as an inductive relation 
+   than as a function. The cases don't overlap, but we don't need
+   to know that at definition time.
+*)
+
+
+(* When does APPLY diverge? (i.e. there is no w, s.t. APPLY D1 D2 w holds)
+    - D1 is empty
+    - D2 is empty
+    - D1 contains a vfun or V ↦ x, but cannot be applied to D2
+           << should this be empty or wrong??? >> 
+
+   When does APPLY propagate wrong?
+    - wrong in D1 or D2  (FUNWRONG / ARGWRONG) 
+    - V ↦ wrong in D1 and valid V in D2  (BETA case)
+
+   When does APPLY create a new wrong? 
+    - D1 contains a successful Value that is not a v_fun, v_map or v_list  (APPWRONG)
+    - D1 contains a v_list and D2 contains a successful Value that is not a nat (PROJWRONG)
+           
+*)
+
+Inductive applicable : Value -> Prop :=
+  | a_fun  : applicable v_fun
+  | a_list : forall VS, applicable (v_list VS)
+  | a_map  : forall V w, applicable (v_map V w).
+
+#[export] Hint Constructors applicable : core.
+
+Inductive APPLY : P Value -> P Value -> (Comp (list Value) -> Prop) :=
+  | BETA : forall D1 D2 w V,
+      (V ↦ w) ∈ D1 ->
+     (mem V ⊆ D2) -> valid_mem V ->
+     APPLY D1 D2 w
+
+(* NOTE: this definition is wrong! need to incorporate eta-expansion here to order for exists
+
+  <v1 ... vn > i == (i=0;v1) | .. | (i=n;vn)
+
+*)
+ 
+  | PROJ   : forall D1 D2 w VS k, 
+     (v_list VS) ∈ D1 ->
+     (v_nat k ∈ D2) -> nth_error VS k = Some w ->
+     APPLY D1 D2 (ret (w  :: nil))
+  | APPWRONG : forall D1 D2 x, 
+      x ∈ D1 ->
+      not (applicable x) ->      
+      APPLY D1 D2 c_wrong
+  | PROJWRONG : forall D1 D2 VS x, 
+     (v_list VS) ∈ D1 ->
+     (x ∈ D2) -> 
+     (forall k, x <> (v_nat k)) ->
+     APPLY D1 D2 c_wrong. 
+
+Infix "▩" := APPLY (at level 90).
+
+#[export] Hint Constructors APPLY : core.
+
+Definition ADD : P Value :=
+  fun w => 
+    match w with 
+    | (V ↦ c_multi (K :: nil)) => 
+        exists i j k, (mem V ≃ ⌈ v_list (v_nat i :: v_nat j :: nil) ⌉) /\ (mem K ≃ ⌈ v_nat k ⌉) /\ (k = i + j)
+    | V ↦ c_wrong => 
+        not (exists i j, v_list (v_nat i :: v_nat j :: nil) ∈ mem V) /\ valid_mem V
+    | _ => False
+    end.
+
+(* ------------------------------------------------------- *)
+
+Definition Rho := Env (P Value).
+
+Definition Bottom : P Value := fun x => False.
+
+Ltac gather_atoms ::=
+  let A := gather_atoms_with (fun x : vars => x) in
+  let B := gather_atoms_with (fun x : var => {{ x }}) in
+  let C := gather_atoms_with (fun x => fv_tm x) in
+  let D := gather_atoms_with (fun x : list (atom * P Value) => dom x) in
+  let E := gather_atoms_with (fun x : Rho => dom x) in
+  constr:(A \u B \u C \u D \u E).
+
+Module EnvNotations.
+Notation "ρ ⋅ x" := (Env.access Bottom ρ x) (at level 50).
+Infix "⊔e" := (Env.map2 Union) (at level 60).
+Infix "⊆e" := (Env.Forall2 Included) (at level 50).
+End EnvNotations.
+Import EnvNotations.
+
+(* ------------------------------------------------------- *)
+
+
+Definition monotone {A}{B} (F : P A -> P B) : Set := 
+  forall D1 D2, (D1 ⊆ D2) -> F D1 ⊆ F D2.
+
+(* aka sub_preserving *)
+Definition sub_reflecting {A}{B} (F : P A -> P B) : Set := 
+  forall D1 D2, F D1 ⊆ F D2 -> (D1 ⊆ D2).
+
+Definition monotone_env {A} (D : Rho -> P A) := 
+  forall ρ ρ' , ρ ⊆e ρ' -> (D ρ) ⊆ D ρ'.
+
+Definition finite {B} (X : P B) : Prop := 
+  exists E, (X ≃ mem E) /\ E <> nil.
+
+Definition finite_env : Rho -> Prop := Env.Forall finite.
+  
+(* ------------------------------------------------------- *)
+
+Definition nonempty_env : Rho -> Type := Env.ForallT nonemptyT.
+
+Definition valid_env : Rho -> Type := Env.ForallT valid. 
+
+Definition sub_env : Rho -> Rho -> Prop := Env.Forall2 Included.
+
+Definition same_env : Rho -> Rho -> Prop := Env.Forall2 Same_set.
+
+(* ------------------------------------------------------- *)
+
+Import LCNotations.
+Open Scope tm.
+
+(* Denotation function *)
+(* `n` is is a termination metric. *)
+Fixpoint denot_comp_n (n : nat) (a : tm) (ρ : Rho) : P (Comp (list Value)) :=
+  let fix denot_val_n (n : nat) (a : tm) (ρ : Rho) : P Value :=
+  match n with
+  | O => fun x => False
+  | S m => 
+     match a with 
+     | var_b _ => fun x => False
+
+     | var_f x => ρ ⋅ x 
+
+     | abs t => 
+        let x := fresh_for (dom ρ \u fv_tm t) in 
+        (Λ (fun D => (denot_comp_n m (t ^ x) (x ~ D ++ ρ))))
+
+     | tcons t u => CONS (denot_val_n m t ρ) (denot_val_n m u ρ)
+
+     | lit k => NAT k
+
+     | add => ADD
+
+     | tnil => NIL
+
+     | _ => fun x => False
+     end
+  end in
+  match n with
+  | O => ∅
+  | S m => 
+      match a with 
+       | app t u   => 
+           BIND (denot_comp_n m t ρ) (fun v1 =>
+           BIND (denot_comp_n m u ρ) (fun v2 =>
+           (v1 ▩ v2)))
+
+       | tcons t u => 
+           BIND (denot_comp_n m t ρ) (fun v1 =>
+           BIND (denot_comp_n m u ρ) (fun v2 => 
+           RET (CONS v1 v2 )))
+
+       | _ => RET (denot_val_n n a ρ)
+     end
+
+  end.
+
+Fixpoint denot_val_n (n : nat) (a : tm) (ρ : Rho) : P Value :=
+  match n with
+  | O => fun x => False
+  | S m => 
+     match a with 
+     | var_b _ => fun x => False
+
+     | var_f x => ρ ⋅ x 
+
+     | abs t => 
+        let x := fresh_for (dom ρ \u fv_tm t) in 
+        (Λ (fun D => (denot_comp_n m (t ^ x) (x ~ D ++ ρ))))
+
+     | tcons t u => CONS (denot_val_n m t ρ) (denot_val_n m u ρ)
+
+     | lit k => NAT k
+
+     | add => ADD
+
+     | tnil => NIL
+
+     | _ => fun x => False
+     end
+  end.
+
+Definition denot (a : tm) := denot_comp_n (size_tm a) a.
+Definition denot_val (a : tm) := denot_val_n (size_tm a) a.
+
+#[export] Hint Opaque denot : core.
+#[export] Hint Opaque denot_val : core.
+
