coq/verse/semantics.v
@@ -1,0 +1,13 @@
+Require Import Coq.Logic.FunctionalExtensionality.
+Require Import Coq.Classes.RelationClasses.
+Require Coq.Relations.Relation_Definitions.
+Require Import Lia.
+
+Require Export lc.tactics.
+Require Import structures.Structures.
+Require Export structures.consistency.
+
+Import MonadNotation.
+Open Scope monad_scope.
+Import SetNotations.
+Local Open Scope set_scope.
