coq/verse/theory_new.v
@@ -1,0 +1,796 @@
+Require Import Coq.Logic.FunctionalExtensionality.
+Require Import Coq.Classes.RelationClasses.
+Require Coq.Relations.Relation_Definitions.
+Require Import Lia.
+
+Require Export lc.tactics.
+Require Import lc.scoped.
+
+Require Import structures.Structures.
+
+Import SetNotations.
+Local Open Scope set_scope.
+Import MonadNotation.
+Open Scope monad_scope.
+
+(* Definitions *)
+Require Import denot.definitions.
+
+(* Rewrite rules for the definition of the denotation *)
+Require Import denot.denot.
+
+(* Weakening *)
+Require Import denot.subst.
+
+(* Operators preserve validity *)
+Require Import denot.valid_theory. 
+
+(* Congruence: operators respect set equality *)
+Require Import denot.congruence_theory.
+
+(* Denotation function is continuous. *)
+Require Import denot.continuity.
+
+(* Denotation produces a consistent set *)
+(* Require Import denot.consistency. *)
+
+Import EnvNotations.
+Import LCNotations.
+Local Open Scope tm.
+
+(* ---- -------------------------------------- *)
+
+(* k∈℘k *)
+Lemma k_in_den_k : forall k, v_nat k ∈ NAT k.
+Proof. intros. reflexivity. Qed.
+
+Lemma k_in_den_k'_inv : forall k k', v_nat k ∈ NAT k' -> k = k'.
+Proof. intros. inversion H. done. Qed.
+
+Lemma v_in_den_k_inv :  forall v k, v ∈ NAT k -> v = v_nat k.
+Proof. intros. destruct v; inversion H. done. Qed.
+
+
+Lemma NAT_den {k} : NAT k ≃ ⌈ v_nat k ⌉.
+split. intros x In. destruct x; try done. inversion In. subst. constructor.
+intros x In. inversion In. cbn. auto. Qed.
+
+Lemma den_list : forall i j D, D ⊆ LIST (NAT i :: NAT j :: nil) ->
+                 forall x, x ∈ D -> x = v_list (v_nat i :: v_nat j :: nil).
+Proof.
+  intros.
+  specialize (H x H0).
+  destruct x; try done. 
+  destruct l; try done; inversion H; subst; clear H.
+  apply v_in_den_k_inv in H4. subst.
+  inversion H6. subst. clear H6.
+  apply v_in_den_k_inv in H2. subst.
+  inversion H4. subst.
+  reflexivity.
+Qed.
+
+Lemma CONS_LIST {k1 k2 } : CONS (NAT k1) (CONS (NAT k2) NIL) ≃ LIST (NAT k1 :: NAT k2 :: nil).
+Proof.
+  intros.
+  split.
+  + intros w In. destruct w; try done.
+    destruct l; try done.
+    destruct In as [x In]. apply v_in_den_k_inv in x.
+    destruct l; try done.
+    destruct In as [y In]. apply v_in_den_k_inv in y.
+    destruct l; try done. 
+    subst. cbn. 
+    econstructor; eauto. reflexivity. 
+    econstructor; eauto. reflexivity. 
+    cbv in In. inversion In.
+  + intros w In.
+    eapply den_list in In. 2: { reflexivity.  }
+    subst. 
+    econstructor; eauto using k_in_den_k.
+    econstructor; eauto using k_in_den_k.
+    econstructor.
+Qed.
+
+Lemma l_equiv_den_k1 {l k} : mem l ≃ ⌈ v_nat k ⌉ -> (mem l ⊆ NAT k) /\ l <> nil.
+Proof.
+  intros.
+  rewrite H.
+  split. rewrite NAT_den. reflexivity.
+  destruct l. cbv in H. destruct H. intro h. eapply (H0 (v_nat k)). eapply in_singleton.
+  done.
+Qed.
+
+Lemma l_equiv_den_k2 {l k} : (mem l ⊆ NAT k) /\ l <> nil -> mem l ≃ ⌈ v_nat k ⌉.
+Proof.
+  move=> [h1 h2].
+  split.
+  rewrite <- NAT_den. done.
+  destruct l. done.
+  have vIn: v ∈ NAT k. eauto.
+  apply v_in_den_k_inv in vIn. subst.
+  eauto.
+Qed.
+
+Lemma l_equiv_den_k {l k} : (mem l ⊆ NAT k) /\ l <> nil <-> mem l ≃ ⌈ v_nat k ⌉.
+Proof. split. eapply l_equiv_den_k2; eauto. eapply l_equiv_den_k1; eauto. Qed.
+
+
+Lemma ADD_APPLY_LIST {i j} : 
+  ADD ▩ (LIST (NAT i :: NAT j :: nil)) ≃ RET (NAT (i + j)).
+Proof.
+  split.
+  + intros w APP. inversion APP; subst; clear APP.
+    all: cbn in H.
+    all: try done.
+    destruct w; try done.
+    - destruct H as [NI VM].
+      assert False. eapply NI. 
+      unfold valid_mem in VM. destruct V; try done.
+      move: (den_list _ _ _ H0 v ltac:(econstructor; eauto)) => h1. 
+      subst.
+      exists i. exists j. eauto. done.
+    - destruct l; try done.
+      destruct l0; try done.
+      destruct H as [i0 [j0 [k0 [h0 [h1 h2]]]]]. subst.
+      cbn.
+      apply l_equiv_den_k1 in h1. destruct h1. 
+      split; eauto.
+      rewrite h0 in H0.
+      move: (den_list _ _ _ H0 (v_list (v_nat i0 :: v_nat j0 :: nil)) ltac:(auto)) => h3. inversion h3. subst. clear h3.
+      auto.
+    - destruct x; try done.
+   + intros w wIn.
+     destruct w; try done.
+     destruct l; try done.
+     destruct l0; try done.
+     cbn in wIn.
+     move: wIn => [wIn VL].
+     have EQ: mem l ≃ ⌈ v_nat (i + j) ⌉. eapply l_equiv_den_k2; eauto.
+     eapply BETA with (V := v_list (v_nat i :: v_nat j :: nil) :: nil).
+     - cbn. exists i. exists j. exists (i+j).
+       repeat split. eauto. eauto.
+       rewrite EQ. eauto.
+       rewrite EQ. eauto.
+     - intros x xIn. inversion xIn. subst.
+       cbn. eauto using k_in_den_k.
+       inversion H.
+     - unfold valid_mem. done. 
+Qed.
+
+Lemma ADD_APPLY_CONS {k1 k2} : 
+  (ADD ▩ CONS (NAT k1) (CONS (NAT k2) NIL)) ≃ RET (NAT (k1 + k2)).
+Proof.
+  rewrite CONS_LIST.
+  eapply ADD_APPLY_LIST.
+Qed. 
+
+Lemma CONS_APPLY_ZERO1 {D1 D2} : (CONS D1 D2 ▩ NAT 0) ⊆ RET D1.
+  intros w APP. inversion APP; try inversion H.
+  + subst.
+    apply v_in_den_k_inv in H0. inversion H0. subst.
+    destruct VS; simpl in H1. done. inversion H1. subst.
+    inversion H.
+    cbn. split.
+Abort.
+(*
+    rewrite <- H2. eauto. 
+    destruct W.  destruct H2 as [h1 h2]. specialize (h1 w0 ltac:(auto)). done.
+    done.
+  + destruct x; try done.
+  + destruct x; try done. 
+    apply v_in_den_k_inv in H0.
+    subst.
+    exfalso. 
+    eapply H1; eauto.
+Qed. *)
+
+Lemma CONS_APPLY_ZERO2 {D1 D2 VS} : 
+  v_list VS ∈ D2 ->
+  RET D1 ⊆ (CONS D1 D2 ▩ NAT 0).
+Proof.
+  intros VV.
+  intros c cIn.
+  destruct c; try done.
+  destruct l; try done.
+  destruct l0; try done.
+  cbn in cIn. move: cIn => [cIn VL].
+  destruct l; try done.
+  have APPW : (forall w, In w l -> v_list (w :: VS) ∈ (CONS D1 D2)).
+Abort.
+(*
+  admit.
+  eapply PROJ with (k := 0)(VS := v :: VS)(w:= a); eauto using k_in_den_k.
+  
+  destruct l.
+  + done.
+  + clear VL.
+    have LH: (v_list (v :: VS) ∈ CONS D1 D2). unfold CONS. cbn; eauto.
+    have EQ: (mem (v :: l) ≃ ⌈ v ⌉). 
+    induction l.  admit.
+    simpl_env. repeat rewrite union_mem.
+    unfold CONS in LH.
+
+    unfold mem.
+    eapply PROJ with (k := 0)(VS := v :: VS)(w:= a); eauto using k_in_den_k.
+  econstructor; eauto.
+Admitted. *)
+
+Lemma CONS_APPLY_ZERO {D1 D2 VS} : v_list VS ∈ D2 -> (CONS D1 D2 ▩ NAT 0) ≃ RET D1.
+Admitted.
+
+Lemma CONS_APPLY_SUCC {D1 D2 VS k} : v_list VS ∈ D2 -> (CONS D1 D2 ▩ NAT (1 + k)) ≃ (D2 ▩ NAT k).
+Admitted.
+
+(*
+Lemma CONS_APPLY_SUCC1 {D1 D2 k} : (CONS D1 D2 ▩ NAT (1 + k)) ⊆ (D2 ▩ NAT k).
+  intros w APP. inversion APP; try inversion H.
+  + subst.
+    apply v_in_den_k_inv in H0. inversion H0. subst.
+    destruct VS; simpl in H1. done. 
+    inversion H.
+    eapply PROJ; eauto using k_in_den_k.
+  + destruct x; try done.
+  + destruct x; try done.
+    exfalso; eapply H2; eauto.
+Qed.
+*)
+
+(* ---------------------------------------------------- *)
+
+(* Nonempty environments *)
+
+Lemma extend_nonempty_env {ρ x X} : 
+  x `notin` dom ρ ->
+  nonemptyT X -> 
+  nonempty_env ρ -> nonempty_env (x ~ X ++ ρ).
+Proof. intros Fr NEP NEX. eapply ForallT_cons; eauto. Qed.
+
+#[export] Hint Resolve extend_nonempty_env : core.
+
+(* ---------------------------------------------------------- *)
+
+(* https://github.com/jsiek/denotational_semantics/blob/master/agda/ISWIMPValue.agda *)
+
+(* ------------------------------------------------------- *)
+
+(* Soundness of reduction with respect to denotation *)
+(* ISWIMPValue.agda *)
+
+Ltac invert_value :=
+  repeat match goal with 
+    | [ H : value (_ _) |- _ ] => inversion H; clear H; subst
+    | [ H : listvalue (_ _) |- _ ] => inversion H; clear H; subst
+  end.
+
+
+Definition valid_Comp (C : P (Comp (list Value))) : Type :=
+  (nonemptyT C * not (c_wrong ∈ C) * not (c_multi nil ∈ C))%type.
+       
+
+Lemma denot_value_valid {t}{ρ} : 
+  fv_tm t [<=] dom ρ -> valid_env ρ 
+  -> (value t -> valid (denot_val t ρ)) * 
+      (listvalue t -> forall (x : Value), x ∈ (denot_val t ρ) -> { l & v_list l = x }).
+Proof.
+  induction t.
+  all: intros FV; simpl in FV.
+  all: intros NEρ.
+  all: split.
+  all: intros h.
+  all: autorewrite with denot.
+  all: try solve [ assert False; invert_value; done].  
+  + unfold valid_env in NEρ.
+    eapply (@ForallT_access _ Bottom _ _) in NEρ.
+    2: instantiate (1:= x); auto.
+    destruct NEρ.
+    exists x0. auto.
+  + pick fresh x.
+    erewrite denot_val_abs with (x:=x); eauto.
+    eapply valid_Λ.
+  + eapply valid_NAT; eauto. 
+  + eapply valid_ADD; eauto.
+  + assert False. inversion h. done.
+  + eapply valid_NIL; eauto.
+  + (* exists nil. cbv. econstructor. *)
+    intros x In. inversion In. exists nil. reflexivity.
+  + simpl in FV. 
+    move: (IHt1 ltac:(fsetdec) NEρ) => [ih11 _].
+    move: (IHt2 ltac:(fsetdec) NEρ) => [ih21 ih22].
+    have V2: value t2. invert_value. auto.
+    have LV: listvalue t2. invert_value. auto.
+    move: (ih21 V2) => [v NW].
+    move: (ih22 LV v NW) => [l le].
+    eapply valid_CONS; eauto. eapply ih11. invert_value. auto.
+    subst. eauto.
+  + move: (IHt1 ltac:(fsetdec) NEρ) => [ih11 _].
+    move: (IHt2 ltac:(fsetdec) NEρ) => [ih21 ih22].
+    have V2: value t2. invert_value. auto.
+    have LV: listvalue t2. invert_value. auto.
+    move: (ih21 V2) => [v  NW].
+    move: (ih22 LV v NW) => [ll ii].
+    subst.
+    intros x CC. 
+    destruct x; try done.
+    exists l. reflexivity.
+Qed.
+
+Lemma denot_val_RET {ρ}{NE: valid_env ρ} {v} : 
+  fv_tm v [<=] dom ρ -> value v -> denot v ρ ≃ RET (denot_val v ρ).
+Proof.
+  induction v.
+  all: intros FV H0.
+  all: inversion H0; try inversion H.
+  all: autorewrite with denot.
+  all: simpl in FV.
+  all: try reflexivity. 
+  rewrite IHv1; eauto.  fsetdec.
+  rewrite BIND_RET.
+  solve_continuous.
+  eapply BIND_CONS_continuous.
+  eapply denot_value_valid; eauto. fsetdec. 
+  rewrite IHv2; eauto. fsetdec.
+  rewrite BIND_RET.
+  solve_continuous.
+  eapply RET_CONS_continuous2.
+  eapply denot_value_valid; eauto. fsetdec. 
+  reflexivity.
+Qed.
+
+Lemma value_nonempty {t}{ρ} : 
+  fv_tm t [<=] dom ρ -> valid_env ρ -> value t -> valid_Comp (denot t ρ).
+Proof. 
+  intros SC VE VT.
+  move: (@denot_val_RET ρ VE t SC VT) => EQ.
+  move: (denot_value_valid SC VE) => [h1 h2].
+  specialize (h1 VT).
+  destruct h1.
+  repeat split.
+  + unfold nonemptyT.
+    exists (c_multi (ret x :: nil)).
+    rewrite EQ.
+    cbn. repeat split; auto. done.
+  + rewrite EQ.
+    cbn. done.
+  + rewrite EQ.
+    cbn. done.
+Qed.
+
+(* Scoping predicates *)
+
+Lemma subst_denot : forall t x u ρ1 ρ2, 
+    scoped t (ρ1 ++ x ~ (denot_val u ρ2) ++ ρ2) ->
+    scoped u ρ2 ->
+    value u ->
+    valid_env (ρ1 ++ ρ2) ->
+    denot t (ρ1 ++ x ~ (denot_val u ρ2) ++ ρ2) ≃
+    denot (t [x ~> u]) (ρ1 ++ ρ2).
+Proof.
+  intro t.
+  eapply tm_induction with (t := t);
+  [move=>i|move=>y|move=>t1 t2 IH1 IH2|move=> t' IH|move=>k| | | move=> t1 t2 IH1 IH2].
+  all: intros x u ρ1 ρ2 ST SU VU NE.
+  all: simpl. 
+  all: simpl_env. 
+  all: autorewrite with denot.
+  all: try solve [reflexivity].
+  + destruct (y == x) eqn:EQ. subst.
+    ++ have NI: x `notin` dom ρ1.
+       { inversion ST. destruct_uniq. auto. }
+       have D2: fv_tm u [<=] dom ρ2. 
+       { inversion SU. auto. }
+       have U2: uniq (ρ1 ++ ρ2). 
+       { inversion ST. solve_uniq. }
+       rewrite access_app_fresh; auto.       
+       rewrite access_eq_var.
+       rewrite denot_val_RET; simpl_env; auto. fsetdec.
+       erewrite weaken_denot_val. reflexivity.
+       fsetdec. auto.
+    ++ repeat rewrite denot_var.
+       eapply Proper_Same_RET; eauto.
+       destruct (access_app_P ρ1 y) as [h1 | h2].
+       repeat rewrite h1. reflexivity.
+       move: (h2 ρ2) => [N1 ->]. 
+       move: (h2 (x ~ denot_val u ρ2 ++ ρ2)) => [N3 ->].
+       rewrite access_neq_var; auto.
+       reflexivity.
+  + move: (scoped_app_inv1 _ _ _ _ ST) => S1.
+    move: (scoped_app_inv2 _ _ _ _ ST) => S2.
+    eapply Proper_Same_BIND.
+    eapply IH1; eauto.
+    intros v1 v2 ->.
+    eapply Proper_Same_BIND.
+    eapply IH2; eauto.
+    intros w1 w2 ->.
+    reflexivity.
+  + have LCU: lc_tm u. inversion SU. auto.
+    pick fresh z.
+    specialize (IH z ltac:(auto) x u).
+    simpl. simpl_env.
+    repeat rewrite (denot_abs z).
+    simpl_env. fsetdec.
+    simpl_env. rewrite fv_tm_subst_tm_upper. fsetdec.
+    eapply Proper_Same_RET.
+    eapply Λ_ext. intros D DV.
+    have FZ: z `notin` (dom (ρ1 ++ x ~ denot_val u ρ2 ++ ρ2) \u fv_tm t').
+    simpl_env. fsetdec. 
+    move: (scoped_abs_inv _ z t' D _ FZ ST) => h.
+    rewrite <- app_assoc.
+    rewrite IH; auto.
+    simpl_env. eapply extend_valid_env; eauto.
+    rewrite subst_tm_open_tm_wrt_tm. eauto.
+    rewrite subst_neq_var. auto.
+    reflexivity.
+  + move: (scoped_tcons_inv1 _ _ _ _ ST) => S1.
+    move: (scoped_tcons_inv2 _ _ _ _ ST) => S2.
+    eapply Proper_Same_BIND.
+    eapply IH1; eauto.
+    intros v' v ->.
+    eapply Proper_Same_BIND.
+    eapply IH2; eauto.    
+    intros w' w ->. 
+    reflexivity.
+Qed.
+
+Lemma subst_denot1 :
+  forall (t : tm) (x : atom) (u : tm) (ρ : Env (P Value)),
+    scoped t (x ~ denot_val u ρ ++ ρ) 
+    -> scoped u ρ 
+    -> value u
+    -> valid_env ρ
+    -> denot t (x ~ denot_val u ρ ++ ρ) ≃ denot (t [x ~> u]) ρ.
+Proof.
+  intros. 
+  eapply subst_denot with (ρ1 := nil); auto. 
+Qed.
+
+
+
+Lemma soundness: 
+  forall t u, 
+    full_reduction t u ->
+    forall ρ,
+    scoped t ρ ->
+    scoped u ρ ->
+    valid_env ρ ->
+    denot t ρ ≃ denot u ρ.
+Proof.
+  intros t u RED. 
+  induction RED; intros ρ SCt SCu NE.
+  all: autorewrite with denot.
+  - (* beta *)
+    destruct SCt as [FV U lc]. inversion lc. subst.
+    simpl in FV.
+    pick fresh x.
+    erewrite denot_abs with (x:=x). 2: fsetdec.
+    rewrite BIND_RET; solve_continuous.
+    eapply valid_Λ; auto.
+    rewrite denot_val_RET; eauto. fsetdec.
+    rewrite BIND_RET; solve_continuous.
+    eapply denot_value_valid; auto. fsetdec.
+    rewrite Λ_denot_APPLY_id; auto.
+    eapply denot_value_valid; auto. fsetdec.
+    rewrite (subst_tm_intro x t v); auto.
+    replace ρ with (nil ++ ρ) at 3.
+    rewrite <- subst_denot with (ρ1 := nil). reflexivity.
+    simpl_env.
+    econstructor; eauto. 
+    rewrite fv_tm_open_tm_wrt_tm_upper. simpl. fsetdec.
+    inversion H; eauto.
+    econstructor; eauto. 
+    fsetdec.
+    auto.
+    auto.
+    reflexivity.
+  - (* abs-cong *)
+    pick fresh x.
+    repeat erewrite denot_abs with (x:=x); try fsetdec.
+    specialize (H0 x ltac:(auto)).
+    eapply Proper_Same_RET.
+    eapply Λ_ext.
+    intros X NEX.
+    eapply H0.
+    have F1 : x `notin` dom ρ \u fv_tm t. fsetdec.
+    eapply (scoped_abs_inv _ x _ X _ F1 SCt).
+    have F2 : x `notin` dom ρ \u fv_tm t'. fsetdec.
+    eapply (scoped_abs_inv _ x _ X _ F2 SCu).
+    eapply extend_valid_env; eauto.
+  - (* app1 *) 
+    have SC1: scoped t ρ. eapply scoped_app_inv1; eauto.
+    have SC2: scoped t' ρ. eapply scoped_app_inv1; eauto.
+    have SC3: scoped u ρ. eapply scoped_app_inv2; eauto.
+    eapply Proper_Same_BIND. eauto.
+    intros v v' ->.
+    eapply Proper_Same_BIND. reflexivity.
+    intros w w' ->.    
+    eapply APPLY_cong. reflexivity. reflexivity.
+  - (* app2 *)
+    have SC1: scoped t ρ.  eapply scoped_app_inv1; eauto.
+    have SC2: scoped u ρ.  eapply scoped_app_inv2; eauto.
+    have SC3: scoped u' ρ.  eapply scoped_app_inv2; eauto.
+    eapply Proper_Same_BIND. reflexivity.
+    intros v v' ->.
+    eapply Proper_Same_BIND. auto.
+    intros w w' ->.    
+    eapply APPLY_cong. reflexivity. reflexivity.
+  - (* cons1 *)
+    have SC1: scoped t ρ.  eapply scoped_tcons_inv1; eauto.
+    have SC2: scoped u ρ.  eapply scoped_tcons_inv2; eauto.
+    have SC3: scoped t' ρ.  eapply scoped_tcons_inv1; eauto.
+    eapply Proper_Same_BIND. eauto.
+    intros v v' ->.
+    eapply Proper_Same_BIND. reflexivity.
+    intros w w' ->.    
+    eapply Proper_Same_RET.
+    eapply CONS_cong. reflexivity. reflexivity.
+  - (* cons2 *)
+    have SC1: scoped t ρ.  eapply scoped_tcons_inv1; eauto.
+    have SC2: scoped u ρ.  eapply scoped_tcons_inv2; eauto.
+    have SC3: scoped u' ρ.  eapply scoped_tcons_inv2; eauto.
+    eapply Proper_Same_BIND. reflexivity.
+    intros v v' ->.
+    eapply Proper_Same_BIND. auto.
+    intros w w' ->.    
+    eapply Proper_Same_RET.
+    eapply CONS_cong. reflexivity. reflexivity.
+  - (* prj_zero *)
+
+    destruct SCt. simpl in s.
+    have Vv : valid (denot_val v ρ). { eapply denot_value_valid; eauto. fsetdec. }
+    move: (@denot_value_valid w ρ ltac:(fsetdec) NE) => [h1 h2]. specialize (h2 H0).
+    have Vw : valid (denot_val w ρ). eauto. 
+    destruct (h1 ltac:(auto)) as [x xIn]. destruct (h2 x xIn) as [l1 <-]. 
+
+    rewrite denot_val_RET; eauto. fsetdec.
+    rewrite BIND_RET; solve_continuous.
+    eapply BIND_continuous; solve_continuous.
+
+    rewrite denot_val_RET; eauto. fsetdec.
+    rewrite BIND_RET; solve_continuous.
+    rewrite BIND_RET; solve_continuous.
+    eapply valid_CONS; eauto.
+
+    rewrite BIND_RET; solve_continuous.
+    eapply valid_NAT.
+
+    eapply CONS_APPLY_ZERO.
+    eauto.
+  - (* prj_suc *)
+
+    destruct SCt. simpl in s.
+    have Vv : valid (denot_val v ρ). { eapply denot_value_valid; eauto. fsetdec. }
+    move: (@denot_value_valid w ρ ltac:(fsetdec) NE) => [h1 h2]. specialize (h2 H0).
+    have Vw : valid (denot_val w ρ). eauto. 
+    destruct (h1 ltac:(auto)) as [x xIn]. destruct (h2 x xIn) as [l1 <-]. 
+
+    rewrite denot_val_RET; eauto. fsetdec.
+    rewrite BIND_RET; solve_continuous.
+    eapply BIND_continuous; solve_continuous.
+
+    rewrite denot_val_RET; eauto. fsetdec.
+    rewrite BIND_RET; solve_continuous.
+    rewrite BIND_RET; solve_continuous.
+    eapply valid_CONS; eauto.
+
+    rewrite BIND_RET; solve_continuous.
+    eapply valid_NAT.
+
+    rewrite BIND_RET; solve_continuous.
+    rewrite BIND_RET; solve_continuous.
+    eapply valid_NAT.
+
+    eapply CONS_APPLY_SUCC.
+    eauto.
+  - (* add *) 
+    rewrite (BIND_RET ADD); solve_continuous.
+    eapply valid_ADD.
+
+    rewrite (BIND_RET (NAT k1)); solve_continuous.
+    eapply BIND_continuous; solve_continuous.
+    eapply valid_NAT.
+
+
+    rewrite (BIND_RET (NAT k2)); solve_continuous.
+    eapply BIND_continuous; solve_continuous.
+    eapply valid_NAT.
+
+
+    rewrite BIND_RET; solve_continuous.
+    eapply valid_NIL.
+
+    rewrite BIND_RET; solve_continuous.
+    eapply valid_CONS. eapply valid_NAT. eapply valid_NIL.
+    instantiate (1:= nil). cbv. econstructor; eauto.
+    
+    rewrite BIND_RET; solve_continuous.
+    eapply valid_CONS. eapply valid_NAT. eapply valid_CONS. eapply valid_NAT. eapply valid_NIL.
+    instantiate (1:= nil). cbv. econstructor; eauto.
+    instantiate (1:= v_nat k2 :: nil). cbv. split. auto. econstructor; eauto.
+    
+    eapply ADD_APPLY_CONS; eauto.
+Qed.
+
+
+(* --------------------------------------------------------------- *)
+
+(* Example semantics *)
+
+(* Prove that 3 + 4 *)
+Definition tm_Add : tm := 
+  app add (tcons (lit 3) (tcons (lit 4) tnil)).
+
+Lemma denot_tm : denot tm_Add nil ≃ RET (NAT 7).
+Proof.
+  unfold tm_Add.
+  autorewrite with denot.
+  
+  rewrite BIND_RET; solve_continuous. eapply valid_ADD.
+  rewrite BIND_RET; solve_continuous. eapply BIND_continuous; solve_continuous. 
+  eapply valid_NAT.
+  rewrite BIND_RET; solve_continuous. eapply BIND_continuous; solve_continuous.
+  eapply valid_NAT.
+  rewrite BIND_RET; solve_continuous. eapply valid_NIL.
+  rewrite BIND_RET; solve_continuous. eapply valid_CONS. eapply valid_NAT. eapply valid_NIL.
+  instantiate (1:=nil). econstructor; eauto.
+  rewrite BIND_RET; solve_continuous. eapply valid_CONS. eapply valid_NAT. 
+  eapply valid_CONS. eapply valid_NAT. eapply valid_NIL.
+  instantiate (1:=nil). econstructor; eauto.
+  instantiate (1:= (v_nat 4 :: nil)). repeat econstructor; eauto.
+
+  rewrite ADD_APPLY_CONS.
+  reflexivity.
+Qed.
+
+Definition tm_Id : tm := abs (var_b 0).
+
+Lemma denot_Id {v} : c_multi (ret (v :: nil ↦ c_multi (ret v :: nil)) :: nil) ∈ denot tm_Id nil.
+Proof.
+  pick fresh x.
+  rewrite (denot_abs x); simpl; auto.
+  cbn.
+  destruct (x == x); try done.
+  split. 2: done.
+  intros y yIn. cbv in yIn. destruct yIn; try done. subst.
+  cbn. 
+  repeat split. reflexivity.
+  done.
+  done.
+Qed. 
+
+(* A term with an unbound variable has no value. *)
+Definition tm_Wrong : tm := app (var_b 1) (var_b 0).
+
+Lemma RET_strict : RET (fun (x : Value) => False) ≃ fun x => False.
+Proof.
+  unfold RET.
+  split.
+  intros x xIn.
+  destruct x; try done.
+  destruct l; try done.
+  destruct l0; try done.
+  destruct xIn.
+  destruct l; try done.
+  specialize (H v ltac:(auto)).  done.
+  intros x xIn. done.
+Qed.
+
+Lemma denot_Wrong : c_wrong ∈ denot tm_Wrong nil.
+Proof.
+  unfold tm_Wrong.
+  rewrite denot_app.
+  repeat rewrite denot_var_b.
+  rewrite -> RET_strict.
+  unfold BIND. 
+  simpl.
+  unfold RET.
+  rewrite BIND_RET; solve_continuous.
+  auto.
+Qed.  
+
+
+Lemma denot_Id_inv : forall x ρ, x ∈ denot tm_Id ρ ->
+                          forall w,  Consistent x (w :: nil ↦ w).
+Proof.
+  intros x ρ.
+  unfold tm_Id. 
+  pick fresh y.
+  rewrite (denot_abs y); auto.
+  intro h. 
+  destruct x; try done.
+  move: h => [h0 [h1 h2]].
+  cbn in h0. rewrite eq_dec_refl in h0.
+  intros w.
+  destruct (dec_con x w). eauto.
+  eapply c_map1.
+  exists x. exists w.
+  
+  repeat split; eauto. 
+  unfold In. eauto.
+Qed.
+
+Definition tm_Delta : tm := abs (app (var_b 0) (var_b 0)).
+
+
+#[global] Hint Rewrite access_eq_var : lngen.
+
+Lemma wrong_not_successful {l}: 
+  Forall success l -> v_wrong ∈ mem l -> False.
+Proof. 
+  induction l; intros h1 h2. done.
+  inversion h1. subst. 
+  inversion h2. subst. done.
+  eauto.
+Qed.
+
+Lemma denot_Delta_inv :
+  forall x, x ∈ denot tm_Delta nil -> 
+       exists v w, Consistent x (((v :: nil ↦ w) :: v :: nil) ↦ w).
+Proof.
+  intro x. unfold tm_Delta.
+  pick fresh y.
+  rewrite (denot_abs y); auto.
+  cbn. rewrite eq_dec_refl.
+  destruct x; try done.
+  move=> [h0 [h1 h2]].
+  - inversion h0; subst; try done.
+    + exfalso. eapply wrong_not_successful; eauto.
+    + exfalso. eapply wrong_not_successful; eauto.
+    + exists (l ↦ x). exists x.
+      eapply c_map2. reflexivity.
+    + exists (l ↦ x). exists x.
+      eapply c_map2. reflexivity.
+    + exists (v_nat 0). exists v_wrong. eauto.
+    + exists (v_nat 0). exists v_wrong. eauto.
+  - cbn. intros.
+      exists v_fun. exists v_fun. eauto.
+Qed.
+
+Lemma denot_Delta : forall (v w : Value), success v ->
+    (((v :: nil ↦ w) :: v :: nil) ↦ w) ∈ denot tm_Delta nil.
+Proof.
+  intros v w NW.
+  pick fresh x.
+  unfold tm_Delta.
+  rewrite (denot_abs x); auto.
+  cbn. rewrite eq_dec_refl.
+  split. 2: { unfold valid_mem. split. intro h. done. 
+              econstructor; eauto. done. }
+  cbv.
+  eapply BETA with (V := v :: nil).
+  unfold In. left. auto.
+  rewrite -> mem_singleton. 
+  intros x0 II. inversion II. subst. cbv. right. left. auto.
+  unfold valid_mem.
+  split; eauto.
+  intro h. done. 
+Qed.
+  
+
+Definition tm_Omega : tm := app tm_Delta tm_Delta.
+
+Lemma denot_Omega : forall v, not (v ∈ denot tm_Omega nil).
+Proof.
+unfold tm_Omega.
+rewrite denot_app.
+intro v.
+intro h.
+inversion h; subst; clear h.
++ apply denot_Delta_inv in H.
+  move: H => [v [w C]]. inversion C.
++ apply denot_Delta_inv in H.
+  move: H => [v [w C]]. inversion C.
++ apply denot_Delta_inv in H.
+  move: H => [v1 [w2 C]]. 
+  inversion C; subst.
+Abort.
+
+
+
+
+
+(* Λ  \Lambda
+   ▩  \squarecrossfill 
+   ↦  \mapsto  
+   ⤇ \Mapsto  
+   ●  \CIRCLE 
+   ⊆  \subseteq   (Included)
+*)
