coq/verse/notes.md
@@ -1,0 +1,191 @@
+NOTES:
+
+* The denotation of the function "\x. if x = 3 then loop else x" is:
+
+         { 1 |-> 1 , 2 |-> 2 , 4 |-> 4 , ... }
+
+  If the function diverges on a particular input there just isn't a result 
+  in the table for that argument.
+
+  On application, this will produce an empty set, because
+  there won't be a matching domain.
+  
+How to represent (finite) choice?
+---------------------------------
+  
+* We have: `one ( v | loop ) = v`
+
+  This example means that we must interpret choose lazily.
+  In other words, if one part of the sequence fails to terminate, then the 
+  rest of the sequence should not be jeopardized.
+  
+* This means that we cannot just add a new constructor
+
+        v_choice : list Value -> Value 
+  
+  to the semantic type `Value` because we cannot represent an infinite loop in
+  the middle of a choice.
+  
+  Instead we need to do something like this to allow divergence inside of 
+  choice. 
+  
+        denot t : list (P Value)
+        denot (v | loop) = [ denot_v v ; {} ]
+        
+  Then, `one` can ignore the diverging term and `all` can detect it and 
+  diverge.
+
+* NOTE: it may be useful to distinguish between the denotation of a value and
+  the denotation of an expression.
+  
+        denot_v t : P Value
+        denot_e t : list (P Value)
+
+* However, functions should be able to go wrong or fail or return 
+  multiple results. What to do?
+  
+Do we need to modify  v_map : Value -> Value -> Value ?
+-------------------------------------------------------
+
+Can we still use the "graph" approximation of functions, even in the presence
+of choice?
+
+* The fact that the denotation of expressions produces a list 
+  means that we need to have this type for LAMBDA:
+
+      LAMBDA : (P Value -> list (P Value)) -> list (P Value)
+
+* We can use the old type for APPLY 
+  
+      APPLY : P Value -> P Value -> P Value
+  
+  For function application, we use bind for CBV
+
+      v1 <- denot e1 ;;
+      v2 <- denot e2 ;;
+      ret (APPLY v1 v2)
+
+  If the denotation of e1 is a list of functions, i.e. functions that 
+  return results
+  
+  This means that we would have the following equation:
+  
+     \x . (e1 | e2) == (\x . e1) | (\x. e2)
+
+  Is that OK? One looks like a single result, and the other looks like 
+  multiple results. 
+  
+* This approach is a bit suspicious. How do we define LAMBDA above?
+  And doesn the equation above require the function to produce the same 
+  set of choices for all arguments?
+
+* Can we denote a function "\x. x | x + 1"  
+
+  A list of sets:
+  
+      [ { 1 |-> 1 , 2 |-> 2 } ; { 1 |-> 2 , 2 |-> 3 , ... }  ]
+
+  A set of lists:
+
+      { [1 |-> 1 ; 1 |-> 2] , [2 |-> 2 ; 2 |-> 3] , ... } ]
+       
+* Can we denote:  "\x.  x | loop | x + 1"
+
+  A list of sets: Yes!
+  
+    [ { 1 |-> 1 , 2 |-> 2 } ; {} ; { 1 |-> 2 , 2 |-> 3 , ... }  ]
+  
+  A set of lists: NO!
+  
+    { [1 |-> 1 ; ??? ; 1 |-> 2] , [2 |-> 2 ; ??? ; 2 |-> 3] , ... }
+
+
+* Can we denote:  `\x.  x | loop | x + 1 | fail`
+
+  A list of sets: Yes! (But, it looks the same as above...)
+  
+        [ { 1 |-> 1 , 2 |-> 2 } ; {} ; { 1 |-> 2 , 2 |-> 3 , ... }  ]
+
+* Can we denote: "\x.fail"  
+
+        [] 
+
+  NOTE: this is the same as "fail"
+  
+        [] 
+
+  But is different from "\x.loop"
+  
+        [ {} ]
+    
+* Can we denot: "\x. x<3" i.e. identity for 0,1,2 but fail for 3 and above?
+ 
+        e1 = [ { 0|->0, 1|->1, 2|->2 } ]
+
+  Is this different from:
+  
+        e2 = [ { 0|->0, 1|->1, 2|->2 } ; {} ]
+
+  If we do an application `e1 3`
+  
+        v1 <- e1
+        v2 <- [ v_nat 0 ] 
+        ret (APPLY v1 v2)
+  
+  The APPLY operation cannot find anything, so returns `[ {} ]`
+  a single diverging value.
+  
+  For the second version `e2 3` we have `[ {} ; {} ]`. That is different
+  but not what we want (i.e. no value `[]` )
+  
+Idea: choice values + choice expressions
+----------------------------------------
+
+What if we add 
+
+      v_multi : list Value -> Value 
+      
+to the domain and use `v_multi []` as the result of failing lambda
+expressions. However, it is the responsibilty of the `return` operation 
+to map `v_multi` into lists.
+
+      return : P Value -> list (P Value)
+
+
+
+
+
+
+
+
+Examples from verse paper:
+
+( 1 | ( 2 | 3 ) ) = ( 1 | 2 | 3 )
+
+
+one ( 1 | loop ) = 1
+
+all ( 1 | loop ) = loop 
+
+
+all ( 1 | 2 | 3 ) = < 1, 2, 3 >
+
+exists x. < 1 , 2, 3 > x = ( 1 | 2 | 3 )
+
+
+(ground) values 
+  v ::= k | op | < v1 ... vn > | \x . e
+
+Rules from verse paper for choice:
+
+one (fail)  = fail
+one (v)     = v
+one (v | e) = v
+all (fail)  = <> 
+all (v1 | .. | vn) = < v1 .. vn >
+fail | e    = e 
+e | fail    = e 
+
+Example with functions/one/choice:
+
+one { (\x. (x | loop) 3 }
